src/tls/Mem.fst
@@ -1,7 +1,9 @@
 module Mem
 
 /// Setting a uniform HyperStack-based memory model, and gathering
-/// abbreviations and top-level regions.
+/// abbreviations and top-level regions. Note this module already
+/// depends on Flags (as we do not wish to extract the global TLS
+/// region and its contents).
 
 open FStar.HyperStack.All
 
@@ -16,6 +18,8 @@ include FStar.HyperStack.ST
 module HH = FStar.HyperHeap // avoid if we can
 module HS = FStar.HyperStack
 //module ST = FStar.HyperStack.ST
+
+let model = Flags.model 
 
 let disjoint = HH.disjoint
 
@@ -74,6 +78,23 @@ let tls_honest_region: r:tls_rgn{r `disjoint` tls_tables_region /\ r `disjoint` 
   match p with | (| _, _, r |) -> r
 
 
+
+
+// used for defining 1-shot PRFs.
+val ssa: #a:Type0 -> Preorder.preorder (option a)
+let ssa #a =
+  let f x y =
+    match x,y with
+    | None, _  -> True
+    | Some v, Some v' -> v == v'
+    | _ -> False in
+  f
+
+
+
+
+(* An earlier variant of the code below, to be deleted 
+
 // FIXME(adl) can't write Set.set rgn because unification fails in pkg!!
 // FIXME(adl) overcomplicated type because of transitive modifications.
 // An rset can be thought of as a set of disjoint subtrees in the region tree
@@ -101,3 +122,99 @@ type disjoint_rset (s1:rset) (s2:rset) =
 assume val lemma_disjoint_ancestors:
   r1:rgn -> r2:rgn -> p1:rgn{r1 `is_below` p1} -> p2:rgn{r2 `is_below` p2}
   -> Lemma (requires p1 <> p2) (ensures HH.disjoint r1 r2 /\ r1 <> r2)
+*)
+
+// FIXME(adl) can't write Set.set rgn because unification fails in pkg!!
+// the second line embeds the definition of rgn because of the unification bug
+// FIXME(adl) overcomplicated type because of transitive modifications.
+// An rset can be thought of as a set of disjoint subtrees in the region tree
+// rset are downward closed - if r is in s and r' extends r then r' is in s too
+// this allows us to prove disjointness with negation of set membership
+
+
+module MR = FStar.Monotonic.RRef
+module MM = FStar.Monotonic.Map
+module MH = FStar.Monotonic.Heap
+
+/// SZ: changed the definition to quantify over [HH.rid] rather than [rgn]
+type rset = s:Set.set HH.rid{
+  (forall (r1:HH.rid). (Set.mem r1 s ==>  //AR: 12/05: Add the pattern (Set.mem r1 s)?
+     r1 <> HH.root /\
+     (is_tls_rgn r1 ==> r1 `HH.extends` tls_tables_region) /\
+     (forall (r':HH.rid).{:pattern (r' `HH.includes` r1)} r' `is_below` r1 ==> Set.mem r' s) /\
+     (forall (r':HH.rid).{:pattern is_eternal_region r'} r' `is_above` r1 ==> is_eternal_region r')))}
+
+let rset_union (s1:rset) (s2:rset)
+  : Tot (s:rset{forall (r:HH.rid). Set.mem r s <==> (Set.mem r s1 \/ Set.mem r s2)}) //AR: 12/05: The refinement is not needed, as Set.union provides this mem property already
+  = Set.union s1 s2
+
+/// SZ: This is the strongest lemma that is provable
+/// Note that this old stronger version doesn't hold:
+///
+/// let lemma_rset_disjoint (s:rset) (r:HH.rid) (r':HH.rid)
+///  : Lemma (requires ~(Set.mem r s) /\ (Set.mem r' s))
+///          (ensures  r `HH.disjoint` r')
+///  = admit() // easy
+///
+let lemma_rset_disjoint (s:rset) (r:HH.rid) (r':HH.rid)
+  : Lemma (requires Set.mem r s /\ ~(Set.mem r' s) /\ r' `is_below` r)
+          (ensures  r `HH.disjoint` r')
+  = ()
+
+// We get from the definition of rset that define_region and tls_honest_region are disjoint
+let lemma_define_tls_honest_regions (s:rset)
+  : Lemma (~(Set.mem tls_define_region s) /\ ~(Set.mem tls_honest_region s))
+  = ()
+
+assume val lemma_disjoint_ancestors:
+  r1:rgn -> r2:rgn -> p1:rgn{r1 `is_below` p1} -> p2:rgn{r2 `is_below` p2}
+  -> Lemma (requires p1 <> p2) (ensures HH.disjoint r1 r2 /\ r1 <> r2)
+
+type trivial_inv (#it:eqtype) (#vt:it -> Type) (m:MM.map' it vt) = True
+type i_mem_table (#it:eqtype) (vt:it -> Type) =
+  MM.t tls_define_region it vt trivial_inv
+type mem_table (#it:eqtype) (vt:it -> Type) =
+  (if model then i_mem_table vt else unit)
+
+let itable (#it:eqtype) (#vt:it -> Type) (t:mem_table vt)
+  : Pure (i_mem_table vt) (requires model) (ensures fun _ -> True) = t
+let mem_addr (#it:eqtype) (#vt:it -> Type) (t:i_mem_table vt)
+  : GTot nat = (HS.as_addr (MR.as_hsref t))
+
+type mem_fresh (#it:eqtype) (#vt:it -> Type) (t:mem_table vt) (i:it) (h:mem) =
+  model ==> MM.fresh (itable t) i h
+type mem_defined (#it:eqtype) (#vt:it -> Type) (t:mem_table vt) (i:it) =
+  model ==> (MR.witnessed (MM.defined (itable t) i))
+type mem_update (#it:eqtype) (#vt:it -> Type) (t:mem_table vt) (i:it) (v:vt i) (h0:mem) (h1:mem) =
+  mem_defined t i /\
+  (model ==> MR.m_sel h1 (itable t) == MM.upd (MR.m_sel h0 (itable t)) i v)
+
+type mem_stable (#it:eqtype) (#vt:it -> Type) (t:mem_table vt) (h0:mem) (h1:mem) =
+  model ==> MR.m_sel h0 (itable t) == MR.m_sel h1 (itable t)
+type mem_empty (#it:eqtype) (#vt:it -> Type) (t:mem_table vt) (h1:mem) =
+  model ==> MR.m_sel h1 (itable t) == MM.empty_map it vt
+
+type modifies_mem_table (#it:eqtype) (#vt:it -> Type) (t:mem_table vt) (h0:mem) (h1:mem) =
+  (if model then
+     (modifies_one tls_define_region h0 h1 /\
+     HS.modifies_ref tls_define_region (Set.singleton (mem_addr (itable t))) h0 h1)
+  else modifies_none h0 h1)
+type mem_disjoint (#it:eqtype) (#vt:it -> Type) (t:mem_table vt)
+  (#it':eqtype) (#vt':it' -> Type) (t':mem_table vt') =
+  model ==> mem_addr (itable t) <> mem_addr (itable t')
+
+let mem_alloc (#it:eqtype) (vt:it -> Type) : ST (mem_table vt)
+  (requires fun h0 -> True)
+  (ensures fun h0 t h1 -> modifies_mem_table t h0 h1 /\ mem_empty t h1)
+  =
+  if model then MM.alloc #tls_define_region #it #vt #trivial_inv else ()
+
+type mem_contains (#it:eqtype) (#vt:it -> Type) (t:mem_table vt) (h:mem) =
+  model ==> h `contains` (MR.as_hsref (itable t))
+let lemma_mem_disjoint_stable (#it:eqtype) (#vt:it -> Type) (t:mem_table vt)
+  (#it':eqtype) (#vt':it' -> Type) (t':mem_table vt') (h0:mem) (h1:mem) : Lemma
+  (requires modifies_mem_table t h0 h1 /\ mem_disjoint t t' /\ mem_contains t h0 /\ mem_contains t' h0)
+  (ensures mem_stable t' h0 h1) = ()
+let lemma_mem_frame (#it:eqtype) (#vt:it -> Type) (t:mem_table vt) (h0:mem) (r:HH.rid) (h1:mem) : Lemma
+  (requires modifies_one r h0 h1 /\ tls_define_region `HH.disjoint` r /\ mem_contains t h0)
+  (ensures mem_stable t h0 h1) = ()
