src/tls/ideal-flags/Flags.fst
@@ -1,18 +1,5 @@
 module Flags
 
-// debug printing flags, one per module
-assume val debug : bool
-assume val debug_CDH : bool
-assume val debug_Epochs : bool
-assume val debug_FFI : bool
-assume val debug_HS : bool
-assume val debug_HSL : bool
-assume val debug_KS : bool
-assume val debug_NGO : bool
-assume val debug_QUIC : bool
-assume val debug_Record : bool
-assume val debug_TLS : bool
-
 assume val model: bool // scaffolding
 assume val ideal_KEF : bool
 assume val ideal_Nonce : bool
@@ -20,3 +7,20 @@ assume val ideal_Sig : bool
 assume val ideal_PMS : bool
 assume val ideal_PRF : bool
 assume val ideal_AEAD: bool
+
+// debug printing flags, one per module; 
+// the refinement enables us to leak secrets for printing.
+
+let real = b:bool {b ==> ~model}
+assume val debug: real 
+assume val debug_CDH: real
+assume val debug_Epochs: real
+assume val debug_FFI: real
+assume val debug_HS: real
+assume val debug_HSL: real
+assume val debug_KS: real
+assume val debug_NGO: real
+assume val debug_QUIC: real
+assume val debug_Record: real
+assume val debug_TLS: real
+
