src/tls/AEAD.Pkg.fst
@@ -1,0 +1,124 @@
+module AEAD.Pkg
+
+// TODO instead: package from a plausible AEAD.fsti, mirroring
+// SecureAPI's one with bytes instead of buffers.
+
+// As a second step, we will restore AEADProvider between the two, and
+// use it to switch to faster, concrete, correct implementations.
+
+// As a verification unit-test, we may also show how to package two
+// instances of AEAD (for both directions) from the same create/coerce
+// on their concatenated keys, in tLS 1.2 style.
+
+open Mem
+open Pkg
+
+module HH = FStar.HyperHeap // I wish we could avoid it once Mem is open.
+
+/// --------------------------------------------------------------------------------------------------
+/// module AEAD
+/// sample generic, agile functionality.
+///
+/// TODO package instead StAE; what to do with the algorithm?
+
+type aeadAlg = | AES_GCM128 | AES_GCM256
+let aeadLen: aeadAlg -> keylen = function
+  | AES_GCM128 -> 32ul
+  | AES_GCM256 -> 48ul
+
+// 17-10-31  this abbreviation breaks typechecking when used; why?
+// unfold type aeadAlgi (#ip:ipkg aeadAlg) (i:ip.t) = a:aeadAlg {a == ip.get_info i}
+
+assume val flag_AEAD: b:bool{b ==> model}
+type idealAEAD = b2t flag_AEAD
+
+type keyrepr a = lbytes (aeadLen a)
+assume new type key (ip: ipkg) (aeadAlg_of_i: ip.t -> aeadAlg) (i:ip.t{ip.registered i}) // abstraction required for indexing
+
+let prf_region: subrgn tls_tables_region = new_region tls_tables_region
+
+let aead_shared_footprint (#ip:ipkg) (#aeadAlg_of_i: ip.t -> aeadAlg) : rset =
+  assume false; // Downward closed
+  Set.singleton prf_region
+
+assume val aead_footprint:
+  #ip:ipkg -> #aeadAlg_of_i: (ip.t -> aeadAlg) -> #i:ip.t{ip.registered i} ->
+  k:key ip aeadAlg_of_i i -> GTot (s:rset{s `Set.disjoint` aead_shared_footprint #ip #aeadAlg_of_i})
+
+// The local AEAD invariant
+assume val aead_inv:
+  #ip:ipkg -> #aeadAlg_of_i: (ip.t -> aeadAlg) -> #i:ip.t{ip.registered i} ->
+  k:key ip aeadAlg_of_i i -> h:mem -> GTot Type0
+
+assume val aead_invariant_framing: ip:ipkg -> aeadAlg_of_i: (ip.t -> aeadAlg) ->
+  i:ip.t{ip.registered i} -> k:key ip aeadAlg_of_i i ->
+  h0:mem -> r:HH.rid -> h1:mem ->
+  Lemma (requires aead_inv k h0 /\ modifies_one r h0 h1
+          /\ ~(r `Set.mem` aead_footprint k) /\ ~(r `Set.mem` aead_shared_footprint #ip #aeadAlg_of_i))
+        (ensures aead_inv k h1)
+
+assume val aead_empty_log: ip: ipkg -> aeadAlg_of_i: (ip.t -> aeadAlg) ->
+  #i: ip.t{ip.registered i} -> a: aeadAlg {a == aeadAlg_of_i i} ->
+  k:key ip aeadAlg_of_i i -> h1:mem -> Type0
+
+assume val aead_empty_log_framing: ip: ipkg -> aeadAlg_of_i: (ip.t -> aeadAlg) ->
+  #i: ip.t{ip.registered i} -> a: aeadAlg {a == aeadAlg_of_i i} ->
+  k:key ip aeadAlg_of_i i -> h0:mem -> r:HH.rid -> h1:mem -> Lemma
+    (requires (aead_empty_log ip aeadAlg_of_i a k h0 /\ modifies_one r h0 h1 /\ ~(r `Set.mem` aead_footprint k)))
+    (ensures (aead_empty_log ip aeadAlg_of_i a k h1))
+
+assume val create_key: ip: ipkg -> aeadAlg_of_i: (ip.t -> aeadAlg) ->
+  i: ip.t{ip.registered i} -> a:aeadAlg {a == aeadAlg_of_i i} ->
+  ST (key ip aeadAlg_of_i i)
+    (requires fun h0 -> model)
+    (ensures fun h0 k h1 -> modifies_none h0 h1 /\ fresh_regions (aead_footprint k) h0 h1
+      /\ aead_empty_log ip aeadAlg_of_i a k h1 /\ aead_inv k h1)
+
+assume val coerceT_key: ip: ipkg -> aeadAlg_of_i: (ip.t -> aeadAlg) ->
+  i: ip.t{ip.registered i /\ (idealAEAD ==> ~(ip.honest i))} ->
+  a:aeadAlg {a == aeadAlg_of_i i} -> keyrepr a ->
+  GTot (key ip aeadAlg_of_i i)
+
+assume val coerce_key: ip: ipkg -> aeadAlg_of_i: (ip.t -> aeadAlg) ->
+  i: ip.t{ip.registered i /\ (idealAEAD ==> ~(ip.honest i))} ->
+  a:aeadAlg {a == aeadAlg_of_i i} -> k0:keyrepr a ->
+  ST (key ip aeadAlg_of_i i)
+    (requires fun h0 -> True)
+    (ensures fun h0 k h1 -> k == coerceT_key ip aeadAlg_of_i i a k0
+      /\ modifies_none h0 h1 /\ fresh_regions (aead_footprint k) h0 h1
+      /\ aead_empty_log ip aeadAlg_of_i a k h1 /\ aead_inv k h1)
+
+let local_ae_pkg (ip:ipkg) (aeadAlg_of_i: ip.t -> aeadAlg) =
+  LocalPkg
+    (key ip aeadAlg_of_i)
+    (fun (i:ip.t) -> a:aeadAlg{a = aeadAlg_of_i i})
+    (fun #_ a -> aeadLen a)
+    idealAEAD
+    (aead_shared_footprint #ip #aeadAlg_of_i)
+    (aead_footprint #ip #aeadAlg_of_i)
+    (aead_inv #ip #aeadAlg_of_i)
+    (aead_invariant_framing ip aeadAlg_of_i)
+    (aead_empty_log ip aeadAlg_of_i)
+    (aead_empty_log_framing ip aeadAlg_of_i)
+    (create_key ip aeadAlg_of_i)
+    (coerceT_key ip aeadAlg_of_i)
+    (coerce_key ip aeadAlg_of_i)
+
+let mp (ip:ipkg) (aeadAlg_of_i: ip.t -> aeadAlg): ST (pkg ip)
+  (requires fun h0 -> True)
+  (ensures fun h0 p h1 ->
+    //17-12-01 we need freshness and emptyness of the new table + local packaging
+    modifies_mem_table p.define_table h0 h1 /\
+    p.package_invariant h1)
+=
+  memoization_ST #ip (local_ae_pkg ip aeadAlg_of_i)
+
+val encrypt:
+  ip:ipkg -> aeadAlg_of_i: (ip.t -> aeadAlg) -> #i:ip.t{ip.registered i} ->
+  k: key ip aeadAlg_of_i i -> nat -> ST nat
+  (requires fun h0 -> aead_inv k h0)
+  (ensures fun h0 c h1 ->
+    modifies (rset_union (aead_footprint k) (aead_shared_footprint #ip #aeadAlg_of_i)) h0 h1
+    /\ aead_inv k h1)
+
+let encrypt _ _ #_ k v = v + 1
