src/tls/Extract0.fst
@@ -1,0 +1,169 @@
+module Extract0
+
+open Mem
+open Pkg
+open Idx 
+open Pkg.Tree
+open KDF // avoid?
+
+module MR = FStar.Monotonic.RRef
+
+/// --------------------------------------------------------------------------------------------------
+/// PSKs, Salt, and Extraction (can we be more parametric?)
+
+assume val flag_KEF0: d:nat -> b:bool{b ==> model /\ flag_KDF d ==> b}
+type idealKEF0 d = b2t (flag_KEF0 d)
+// to be refined. When exactly do we we switch KEF0? (after KDF0?)
+assume val lemma_kdf_kef0: d:nat -> Lemma (idealKDF d ==> idealKEF0 d)
+
+let safeKEF0 (d:nat) (i:regid) = idealKEF0 d /\ honest i
+
+/// key-derivation table (memoizing create/coerce)
+
+
+// temporary
+let there = Mem.tls_tables_region
+
+// memoizing a single extracted secret
+// now [private] anymore because of its reuse in Extract2.
+type mref_secret (d:nat) (u: usage d) (i: regid) =
+  // would prefer: HyperStack.mref (option (secret u i)) (ssa #(secret u i))
+  MR.m_rref there (option (secret d u i)) ssa
+
+/// covering two cases: application PSK and resumption PSK
+/// (the distinction follow from the value of i)
+type psk (d:nat) (u: usage d) (i: (Idx?.t ii) {ii.registered i}) =
+  ir_key (safeKEF0 d) (mref_secret d u i) (real_secret i) i
+
+let psk_ideal (#d:nat) (#u: usage d) (#i:regid) (p:psk d u i {safeKEF0 d i}): mref_secret d u i =
+  let t : s:ideal_or_real (mref_secret d u i) (real_secret i) {safeKEF0 d i <==> Ideal? s} = p in
+  Ideal?.v t
+
+let ideal_psk (#d:nat) (#u: usage d) (#i:regid) (t: mref_secret d u i{safeKEF0 d i}) : psk d u i =
+  let t : s:ideal_or_real (mref_secret d u i) (real_secret i) {safeKEF0 d i <==> Ideal? s} = Ideal t in
+  assert(model); t
+
+let psk_real (#d:nat) (#u: usage d) (#i:regid) (p:psk d u i {~(safeKEF0 d i)}): real_secret i =
+  lemma_honest_corrupt i;
+  if model then
+    let t : s:ideal_or_real (mref_secret d u i) (real_secret i) {safeKEF0 d i <==> Ideal? s} = p in
+    Real?.v t
+  else p
+
+let real_psk (#d:nat) (#u: usage d) (#i:regid) (t: real_secret i{~(safeKEF0 d i)}) : psk d u i =
+  if model then
+    (lemma_honest_corrupt i;
+    let s : s:ideal_or_real (mref_secret d u i) (real_secret i) {safeKEF0 d i <==> Ideal? s} = Real t in s)
+  else t
+
+type ext0 (d:nat) (u:usage d) (i:id {registered i}) =
+  _:unit{registered (Derive i "" Extract)} & psk d u (Derive i "" Extract)
+
+#set-options "--lax" //17-12-08 until KDF converges
+
+
+val coerceT_psk:
+  #d: nat ->
+  #u: usage d ->
+  i: id {registered i /\ ~(safeKEF0 d i)} ->
+  a: info {a == get_info i} ->
+  raw: lbytes (secret_len a) ->
+  GTot (ext0 d u i)
+let coerceT_psk #d #u i a raw =
+  real_psk #d #u #(Derive i "" Extract) raw
+
+val coerce_psk:
+  #d: nat ->
+  #u: usage d ->
+  i: id {registered i /\ ~(safeKEF0 d i)} ->
+  a: info {a == get_info i} ->
+  raw: lbytes (secret_len a) ->
+  ST (ext0 d u i)
+  (requires fun h0 -> True)
+  (ensures fun h0 k h1 -> k == coerceT_psk #d #u i a raw)
+
+let coerce_psk #d #u i a raw =
+  let i', honest' = register_derive i "" Extract in
+  lemma_corrupt_invariant i "" Extract;
+  (| (), real_psk #d #u #i' raw |)
+
+val create_psk:
+  #d: nat ->
+  #u: usage d ->
+  i: id {registered i} ->
+  a: info {a == get_info i} ->
+  ST (ext0 d u i)
+  (requires fun h0 -> True)
+  (ensures fun h0 p h1 -> (*TBC*) True)
+
+let create_psk #d #u i a =
+  let i', honest' = register_derive i "" Extract in
+  lemma_corrupt_invariant i "" Extract;
+  if flag_KEF0 d && honest' then
+    let t' = secret d u i' in
+    let r: mref_secret d u i' = MR.m_alloc #(option t') #(ssa #t') there None in
+    (| (), ideal_psk #d #u #i' r |)
+  else
+    (| (), real_psk #d #u #i' (sample (secret_len a)) |)
+
+let local_ext0_pkg (d:nat) (u:usage d) : local_pkg ii =
+  LocalPkg
+    (fun (i:id{registered i}) -> ext0 d u i)
+    (fun i -> a: info{a == get_info i})
+    (fun #_ a -> secret_len a)
+    (idealKEF0 d)
+    (Set.empty <: rset)
+    (fun #i (k:ext0 d u i) -> Set.empty)
+    // local invariant
+    (fun #_ k h -> True)
+    (fun r i h0 k h1 -> ())
+    // create/coerce postcondition
+    (fun #_ _ _ _ -> True) // no post-condition
+    (fun #_ _ _ _ _ _ -> ())
+    (create_psk #d #u)
+    (coerceT_psk #d #u)
+    (coerce_psk #d #u)
+
+let pskp (d:nat) (u:usage d): ST (pkg ii)
+  (requires fun h0 -> True)
+  (ensures fun h0 p h1 -> (*TBC*) True)
+  =
+  memoization_ST (local_ext0_pkg d u)
+
+/// HKDF.Extract(key=0, materials=k) idealized as a (single-use) PRF,
+/// possibly customized on the distribution of k.
+val extract0:
+  #d: nat ->
+  #u: usage d ->
+  #i: regid ->
+  k: ext0 d u i ->
+  a: info {a == get_info i} ->
+  ST
+    (secret d u (Derive i "" Extract))
+    (requires fun h0 -> True)
+    (ensures fun h0 p h1 -> (*TBC*) True)
+
+let extract0 #d #u #i k a =
+  let (| _, p |) = k in
+  let i':regid = Derive i "" Extract in
+  let honest' = get_honesty i' in
+  lemma_kdf_kef0 d;
+  if flag_KEF0 d && honest'
+  then
+    let k: mref_secret d u i' = psk_ideal p in
+    match MR.m_read k with
+    | Some extract -> extract
+    | None ->
+      let extract = create d u i' a in
+      let mrel = ssa #(secret d u i') in
+      let () =
+        MR.m_recall k;
+        let h = get() in
+        assume (MR.m_sel h k == None); // TODO framing of call to create
+        assume (mrel None (Some extract)); // TODO Fix the monotonic relation
+        MR.m_write k (Some extract) in
+      extract
+  else
+    let k = psk_real p in
+    let raw = HKDF.extract #(a.ha) (Hashing.zeroHash a.ha) k in
+    coerce d u i' a raw
