src/tls/Extract1.PRF.fst
@@ -1,0 +1,149 @@
+module Extract1.PRF
+
+open Mem
+open Pkg
+open Idx 
+open Pkg.Tree
+open KDF // avoid?
+
+module MR = FStar.Monotonic.RRef
+
+/// The "salt" is an optional secret used (exclusively) as HKDF
+/// extraction key. The absence of salt (e.g. when no PSK is used) is
+/// handled using a special, constant salt marked as compromised.
+///
+/// salt is indexed by the usage of the secret that will be extracted
+/// (the usage of the salt itself is fixed).
+///
+/// We use separate code for salt1 and salt2 because they are
+/// separately idealized (salt1 is more complicated)
+
+assume val flag_PRF1: d:nat -> b:bool{Extract0.flag_KEF0 d ==> b /\ b ==> model}
+let idealPRF1 (d:nat) = b2t (flag_PRF1 d)
+let lemma_kdf_prf1 (d:nat) : Lemma (idealKDF d ==> idealPRF1 d) = admit()
+
+type safePRF1 (d:nat) (i:regid) = idealPRF1 d /\ honest i
+
+assume type salt (d:nat) (u: usage d) (i: id)
+
+assume val create_salt:
+  #d: nat ->
+  #u: usage d ->
+  i: id ->
+  a: info ->
+  salt d u i
+
+assume val coerce_salt:
+  #d: nat ->
+  #u: usage d ->
+  i: id ->
+  a: info ->
+  raw: lbytes (secret_len a) ->
+  salt d u i
+
+#set-options "--lax" 
+
+let local_salt_pkg (d:nat) (u:usage d) : local_pkg ii =
+  LocalPkg
+    (salt d u)
+    (fun (i:id{registered i}) -> a:info{a == get_info i})
+    (fun #_ a -> secret_len a)
+    (idealPRF1 d)
+    // local footprint
+    (Set.empty <: rset)
+    (fun #i (k:salt d u i) -> Set.empty)
+    // local invariant
+    (fun #_ k h -> True)
+    (fun r i h0 k h1 -> ())
+    // create/coerce postcondition
+    (fun #_ _ _ _ -> True) // no post-condition
+    (fun #_ _ _ _ _ _ -> ())
+    (create_salt #d #u)
+    (magic ())
+    (coerce_salt #d #u)
+
+let saltp (d:nat) (u:usage d) : ST (pkg ii)
+  (requires fun h0 -> True)
+  (ensures fun h0 s h1 -> True)
+  =
+  memoization_ST (local_salt_pkg d u)
+
+
+/// HKDF.Extract(key=s, materials=dh_secret) idealized as 2-step
+/// (KEF-ODH, KEF-Salt game); we will need separate calls for clients
+/// and servers.
+
+/// two flags; we will idealize ODH first
+assume val flag_ODH: d:nat -> b:bool { flag_PRF1 d ==> b /\ b ==> model}
+type idealODH (d:nat) = b2t (flag_ODH d)
+type safeODH (d:nat) (i:regid) = idealODH d /\ honest i
+
+
+/// we write prf_ for the middle salt-keyed extraction, conditionally
+/// idealized as a PRF keyed by salt1 depending on flag_prf1
+///
+/// its interface provides create, coerce, leak, and extract its
+/// internal table memoizes it either with *wide* domain gZ, or with
+/// *narrow* domain idh
+///
+/// Returns a narrow-indexed key,
+///
+/// its internal state ensures sharing
+
+assume val prf_leak:
+  #d: nat ->
+  #u: usage d ->
+  #i: regid ->
+  #a: info {a == get_info i} ->
+  s: salt d u i {~(safePRF1 d i)} ->
+  Hashing.Spec.hkey a.ha
+
+type ext1 (d:nat) (u:usage d) (i:regid) (idh:id_dhe) =
+  _:unit{registered (Derive i "" (ExtractDH idh))} &
+  secret d u (Derive i "" (ExtractDH idh))
+
+val prf_extract1:
+  #d: nat ->
+  #u: usage d ->
+  #i: regid ->
+  a: info {a == get_info i} ->
+  s: salt d u i ->
+  idh: id_dhe{~(honest_idh (ExtractDH idh))} ->
+  gZ: bytes ->
+  ST (ext1 d u i idh)
+  (requires fun h0 -> True)
+  (ensures fun h0 k h1 -> True)
+
+let prf_extract1 #d #u #i a s idh gZ =
+  let j, honest' = register_derive i "" (ExtractDH idh) in
+  lemma_corrupt_invariant i "" (ExtractDH idh);
+  let honest = get_honesty i in
+  lemma_kdf_prf1 d;
+  if flag_PRF1 d && honest
+  then
+    // This is the narrow idealized variant--see paper for additional
+    // discussion. Note the algorithm is determined by the salt index.
+    //
+    (| (), create d u j a |)
+    //
+    // We use the define table of the derived KDF to represent the
+    // state of the PRF.  todo: guard [create] with a table lookup;
+    // informally, when calling [prf_extract1] we don't care about the
+    // state of the KDF, as long as it meets its invariant.
+    //
+    // The wide idealized variant is as follows:
+    //
+    // let j0 =
+    //   match Map.find !s.wide (i,gZ) with
+    //   | Some j0 -> j0
+    //   | None    -> s.wide := !s.wide ++ ((i,gZ), length !s.wide) in
+    // JKDF.create u j j0 a
+    //
+    // or just
+    // JKDF.create u j (i,gZ) a
+  else
+    let raw_salt = prf_leak #d #u #i #a s in
+    let raw = HKDF.extract raw_salt gZ in
+    (| (), coerce d u j a raw |)
+    // we allocate a key at a narrow index, possibly re-using key
+    // materials if there are collisions on gZ or raw_salt
