src/tls/Extract1.fst
@@ -1,0 +1,123 @@
+module Extract1
+
+open Mem
+open Pkg
+open Idx 
+open Pkg.Tree
+open KDF // avoid?
+
+module MR = FStar.Monotonic.RRef
+module MM = FStar.Monotonic.Map
+
+// for now 
+open Extract1.PRF
+open Extract1.ODH
+
+// TODO: instead of CommonDH.keyshare g, we need an abstract stateful
+// [abstract type private_keyshare g = mref bool ...] that enables
+// calling it exactly once
+
+/// Initiator computes DH keyshare, irrespective of the KDF & salt.
+let initI (g:CommonDH.group) = odh_init g
+
+/// Responder computes DH secret material
+val extractR:
+  #d: nat ->
+  #u: usage d ->
+  #i: regid ->
+  s: salt d u i ->
+  a: info {a == get_info i} ->
+  gX: odhid ->
+  ST (i_gY: peer_index gX{dfst i_gY == i} & peer_instance i_gY)
+  (requires fun h0 -> True)
+  (ensures fun h0 _ h1 -> True)
+
+let extractR #d #u #i s a gX =
+  let b = if model then CommonDH.is_honest_dhi gX else false in
+  if b then
+   begin
+    let t: odh_table = odh_state in
+    (if None? (MM.lookup t gX) then
+      let peers = MM.alloc #there #(peer_index gX) #(peer_instance #gX) #(fun _ -> True) in
+      let h = get() in
+      assume(None? (MM.sel (MR.m_sel h t) gX));
+      MM.extend t gX peers;
+      assume(MR.stable_on_t t (MM.defined t gX));
+      MR.witness t (MM.defined t gX));
+    odh_test a s gX
+   end
+  else
+   begin
+    // real computation: gY is honestly-generated but the exchange is doomed
+    let gY, gZ = CommonDH.dh_responder (dfst gX) (dsnd gX) in
+    let idh = IDH gX gY in
+    assume(~(honest_idh (ExtractDH idh))); // FIXME
+    let (| _ , k |) : ext1 d u i idh = prf_extract1 a s idh gZ in
+    let k : secret d u (Derive i "" (ExtractDH idh)) = k in
+    let i_gY : peer_index gX = (| i, gY |) in
+    let s : peer_instance #gX i_gY = admit() in
+    (| i_gY, s |)
+   end
+
+(*)
+     let gX : CommonDH.dhi = (| g, CommonDH.ipubshare x |) in
+     CommonDH.honest_dhi gX /\ odh_defined gX
+     /\ (model ==> (CommonDH.fresh_dhr #gX gY h0)))
+*)
+
+/// Initiator computes DH secret material
+val extractI:
+  #d: nat ->
+  #u: usage d ->
+  #i: regid ->
+  a: info {a == get_info i} ->
+  s: salt d u i ->
+  g: CommonDH.group ->
+  x: CommonDH.ikeyshare g ->
+  gY: CommonDH.rshare g (CommonDH.ipubshare x) ->
+  ST(_:unit{registered (Derive i "" (ExtractDH (idh_of x gY)))}
+    & secret d u (Derive i "" (ExtractDH (idh_of x gY))))
+  (requires fun h0 ->
+    let gX : CommonDH.dhi = (| g, CommonDH.ipubshare x |) in
+    CommonDH.honest_dhi gX /\ odh_defined gX)
+  (ensures fun h0 k h1 -> True)
+
+let extractI #d #u #i a s g x gY =
+  let gX: CommonDH.dhi = (| g, CommonDH.ipubshare x |) in
+  let b = if model then CommonDH.is_honest_dhi gX else false in
+  if b then
+    let t: odh_table = odh_state in
+    MR.testify(MM.defined t gX);
+    let peers = Some?.v (MM.lookup t gX) in
+    let idh = IDH gX gY in
+    let i' = Derive i "" (ExtractDH idh) in
+    assume(registered i');
+    assert(wellformed_id i);
+    assume(wellformed_id i'); //17-11-01 same as above?
+    let i_gY : peer_index gX = (| i, gY |) in
+    let ot = secret d u i' in
+    assume ((| d, u |) == u_of_i i); //17-11-01 indexing does not cover u yet
+    let o : option ot = MM.lookup peers i_gY in
+    match o with
+    | Some k -> (| (), k |)
+    | None -> assume false; //17-11-22 why?
+           odh_prf #d #u #i a s g x gY
+  else odh_prf #d #u #i a s g x gY
+
+val extractP:
+  #d: nat ->
+  #u: usage d ->
+  #i: regid ->
+  a: info {a == get_info i} ->
+  s: salt d u i ->
+  ST(_:unit{registered (Derive i "" (ExtractDH NoIDH))}
+    & secret d u (Derive i "" (ExtractDH NoIDH)))
+  (requires fun h0 -> True)
+  (ensures fun h0 r h1 -> True)
+
+let extractP #d #u #i a s =
+  let gZ = Hashing.Spec.zeroHash a.ha in
+   let (| _, k |) = prf_extract1 a s NoIDH gZ in
+   assert(registered (Derive i "" (ExtractDH NoIDH)));
+   let k : secret d u (Derive i "" (ExtractDH NoIDH)) = k in
+   (| (), k |)
