src/tls/Handshake.Secret.fst
@@ -1,0 +1,1523 @@
+module Handshake.Secret.fst
+
+// used to be KeySchedule
+
+open FStar.Heap
+open FStar.HyperHeap
+open FStar.HyperStack
+open FStar.Seq
+open FStar.Set
+
+open Platform.Bytes
+open Platform.Error
+open TLSError
+open TLSConstants
+open Extensions
+open TLSInfo
+open StatefulLHAE
+open HKDF
+open PSK
+
+module MM = FStar.Monotonic.Map
+module MR = FStar.Monotonic.RRef
+module HH = FStar.HyperHeap
+module HS = FStar.HyperStack
+module ST = FStar.HyperStack.ST
+module H = Hashing.Spec
+
+(* A flag for runtime debugging of computed keys.
+   The F* normalizer will erase debug prints at extraction
+   when this flag is set to false *)
+let discard (b:bool): ST unit (requires (fun _ -> True))
+ (ensures (fun h0 _ h1 -> h0 == h1)) = ()
+let print s = discard (IO.debug_print_string ("KS | "^s^"\n"))
+unfold let dbg : string -> ST unit (requires (fun _ -> True))
+  (ensures (fun h0 _ h1 -> h0 == h1)) =
+  if Flags.debug_KS then print else (fun _ -> ())
+
+
+// parsed handshake message transcript; essentially opaque/ghost to
+// the key-schedule: what we get out of HandshakeLog.
+
+type transcript = HandshakeLog.hs_transcript  // ghost 
+let digest (i:id) (t:transcript) = 
+  let ha = ha_of_id i in 
+  let v = HandshakeLog.transcript_bytes t in 
+  t: Hashing.Spec.anyTag {Hashing.CRF.hashed ha v /\ t = Hashing.hash ha v}
+
+
+/// THE LIVE OF KEY INDEXES. we use relative paths to index various
+/// secrets and keys as we progress in the schedule; we try to keep
+/// the index syntax abstract outside this module.
+///
+/// TODO would a bespoke IK.id for TLS help?
+
+let binder_label i = if Preshared? i then "ext binder" else "res binder" 
+let salt_of_ms i = Derive i "derived"     Expand // extraction salt
+
+let ems_of_psk i     = Derive i "" Extract 
+let hms_of_ems i idh = Derive (salt_of_ms i) "" (ExtractDH idh)
+let ams_of_hms i     = Derive (salt_of_ms i) "" Extract 
+
+assume val tmp: Hashing.Spec.anyTag 
+// the branch on the static label will require two UFCMA packages for binders 
+let bns_of_ems i transcript = Derive i (binder_label i) Expand
+let x0s_of_ems i transcript = Derive i "e exp master" (ExpandLog transcript tmp) 
+
+let x1s_of_ams i transcript = Derive i "exp master"   (ExpandLog transcript tmp) 
+let rms_of_ams i transcript = Derive i "res master"   (ExpandLog transcript tmp) 
+
+let psk_of_rms i nonce = Derive i "resumption" (ExpandLog nonce tmp) // ticket-based
+
+// transport secrets have a designated sender role, controlling the
+// reader/writer flag of derived StreamAE instances.
+let rec sender_of_id i = 
+  match i with 
+  | Derive i "c e traffic"  (ExpandLog _ _) 
+  | Derive i "c hs traffic" (ExpandLog _ _) 
+  | Derive i "c ap traffic" (ExpandLog _ _) -> Some Client
+  | Derive i "s hs traffic" (ExpandLog _ _) 
+  | Derive i "s ap traffic" (ExpandLog _ _) -> Some Server
+  | Derive i "traffic upd" Expand -> sender_of_id i
+  | _ -> None 
+let ts_id = i:pre_id {Some? (sender_of_id i)}
+
+let ets_of_ems i transcript: i:ts_id {sender_of_id i = Some Client} = Derive i "c e traffic"  (ExpandLog transcript tmp)
+let cts_of_hms i transcript: i:ts_id {sender_of_id i = Some Client} = Derive i "c hs traffic" (ExpandLog transcript tmp)
+let sts_of_hms i transcript: i:ts_id {sender_of_id i = Some Server} = Derive i "s hs traffic" (ExpandLog transcript tmp)
+let cts_of_ams i transcript: i:ts_id {sender_of_id i = Some Client} = Derive i "c ap traffic" (ExpandLog transcript tmp)
+let sts_of_ams i transcript: i:ts_id {sender_of_id i = Some Server} = Derive i "s ap traffic" (ExpandLog transcript tmp)
+
+//TODO define [aeadAlg_of_i] specifically on transport secrets. 
+//TODO make the most of welldefined_id
+
+let iv_of_ts  (i: ts_id)        = Derive i "iv"          Expand // AEAD static IV
+let key_of_ts (i: ts_id)        = Derive i "key"         Expand // AEAD keying
+let ts_of_ts  (i: ts_id): ts_id = Derive i "traffic upd" Expand // post-handshake rekeying 
+
+// we have three derived MACs for Binders for Finished messages. 
+let fnk_of_s i = Derive i "finished"    Expand // binder/finished MAC keying (not always a ts)
+let bfk_of_ems i transcript = fnk_of_s (bns_of_ems i transcript)
+let cfk_of_hms i transcript = fnk_of_s (cts_of_hms i transcript)
+let sfk_of_hms i transcript = fnk_of_s (sts_of_hms i transcript)
+
+
+#set-options "--lax"
+
+// move to CommonDH?
+let sprint_share (#g:CommonDH.group) (s:CommonDH.pre_share g): string
+  =
+  let kb = CommonDH.serialize_raw #g s in
+  let kh = Platform.Bytes.hex_of_bytes kb in
+  "Share: "^kh
+
+
+//17-12-07 out of date?
+(********************************************
+*    Resumption PSK is disabled for now     *
+*********************************************
+
+abstract type res_psk (i:rmsId) =
+  b:bytes{exists i.{:pattern index b i} index b i <> 0z}
+
+abstract type res_context (i:rmsId) =
+  b:bytes{length b = CoreCrypto.H.tagLen (rmsId_hash i)}
+
+private type res_psk_entry (i:rmsId) =
+  (res_psk i) * (res_context i) * ctx:psk_context * leaked:(rref tls_tables_region bool)
+
+let res_psk_injective (m:MM.map' rmsId res_psk_entry) =
+  forall i1 i2.{:pattern (MM.sel m i1); (MM.sel m i2)}
+       i1 = i2 <==> (match MM.sel m i1, MM.sel m i2 with
+                  | Some (psk1, _, _, _), Some (psk2, _, _, _) -> b2t (equalBytes psk1 psk2)
+                  | _ -> True)
+
+let res_psk_table : MM.t tls_tables_region rmsId res_psk_entry res_psk_injective =
+  MM.alloc #TLSConstants.tls_tables_region #rmsId #res_psk_entry #res_psk_injective
+
+let registered_res_psk (i:rmsId) (h:HH.t) =
+  b2t (Some? (MM.sel (MR.m_sel h res_psk_table) i))
+
+let res_psk_context (i:rmsId{registered_res_psk i}) =
+  let (_, _, c, _) = Some.v (MM.sel res_psk_table i) in c
+
+private let res_psk_value (i:rmsId{registered_res_psk i}) =
+  let (psk, _, _, _) = Some.v (MM.sel res_psk_table i) in psk
+
+**)
+
+
+// PSK (internal/external multiplex, abstract)
+// Note that application PSK is externally defined but should
+// be idealized together with KS
+
+
+/// 17-12-07 this is too abstract to recover packaged key types; the
+/// plan is to recover that information (using ==) for more specific
+/// types of secrets.
+type secret (i:id) = IK.secret (u_of_i i) i
+
+/// for readability so far; we could be more specific
+type ems_id = id
+type hms_id = id
+type ams_id = id 
+
+/// To be refined with whatever it takes to use it as an application
+/// master secret, etc.
+type ems (i:ems_id) = secret i
+type hms (i:hms_id) = secret i
+type ams (i:ams_id) = secret i
+
+(*
+type hsId       = i: id {labelled i ""}
+type asId       = i: id {labelled i ""}
+type finishedId = i: id {labelled i "finished"} 
+type binderId   = i: id {labelled i "ext binder" \/ labelled i "res binder" }
+type rmsId      = i: id {True}
+type exportId = id
+*)
+
+
+type psk (i:id) //TODO from PSK and IK
+
+// We treat the absence of PSK using reserved, corrupt PSK identifiers
+// with all-zero coerced keys.
+
+assume val no_psk_id: IK.kdfa -> i:esId {match i with Preshared ha _ -> True | _ -> False}
+assume val no_psk (i:id): bool
+
+let dummy_psk ha: psk (no_psk_id ha) = 
+  magic() // PSK.coerce (no_psk_id ha) ha (H.zeroHash ha) 
+  // we'll need them to be registered as corrupt and pre-defined to
+  // meet coerce's precondition.
+
+
+/// Move to PSK? DB lookup from concrete pskid to indexed abstract psk & info.
+
+let read_psk (pi:PSK.pskid): ST (i:esId & u:PSK.pskInfo {ha_of_id i = u.early_hash} * psk i)
+  (requires fun h -> True)
+  (ensures fun h0 _ h1 -> modifies_none h0 h1)
+=
+  magic()
+  (*
+  let c = PSK.psk_info pi in
+  let i =
+    if Some? c.ticket_nonce then
+      let (| li, rmsid |) = Ticket.dummy_rmsid c.early_ae c.early_hash in
+      ResumptionPSK #li rmsid
+    else
+      ApplicationPSK #c.early_hash #c.early_ae pi
+    in
+  (id, c, PSK.psk_value pi)
+  *)
+
+(* 17-12-04 now handled within IK/Extract? 
+// Resumption context
+let rec esId_rc : (esId -> St bytes) =
+  function
+  | NoPSK h -> H.zeroHash h
+
+and hsId_rc : (hsId -> St bytes) = function
+  | HSID_DHE (Salt i) _ _ _ -> secretId_rc i
+  | HSID_PSK (Salt i) -> secretId_rc i
+
+and asId_rc : (asId -> St bytes) = function
+  | ASID (Salt i) -> secretId_rc i
+
+and secretId_rc : (secretId -> St bytes) = function
+  | EarlySecretID i -> esId_rc i
+  | HandshakeSecretID i -> hsId_rc i
+  | ApplicationSecretID i -> asId_rc i
+*)
+
+
+// miTLS 0.9:
+// ==========
+// PRF (type pms) -> TLSInfo (type id) -> KEF (extract pms)
+//                     \ StatefulLHAE (coerce id) /
+// TODO rework old 1.2 types
+type ms = bytes
+type pms = bytes
+//17-12-07 can they also be products of IK? no immediate need
+
+// only for TLS 1.3, will need refining 
+let fink (i: id) = HMAC.UFCMA.key IK.ii i
+let binderKey (i: id) = HMAC.UFCMA.key IK.ii i
+//was:
+//type fink (i:finishedId)    = HMAC.UFCMA.key (HMAC.UFCMA.HMAC_Finished i) (fun _ -> True)
+//type binderKey (i:binderId) = HMAC.UFCMA.key (HMAC.UFCMA.HMAC_Binder i) (fun _ -> True)
+
+
+// type exportKey = (i:id & ems i * logInfo)
+
+// Note from old miTLS (in TLSInfo.fst)
+// type id = {
+//  msId   : msId;            // the index of the master secret used for key derivation
+//  kdfAlg : kdfAlg_t;          // the KDF algorithm used for key derivation
+//  pv     : protocolVersion; // should be part of aeAlg
+//  aeAlg  : aeAlg;           // the authenticated-encryption algorithms
+//  csrConn: csRands;         // the client-server random of the connection
+//  ext: negotiatedExtensions;// the extensions negotiated for the current session
+//  writer : role             // the role of the writer
+//  }
+
+
+type ks_alpha12 = 
+  pv:protocolVersion * 
+  cs:cipherSuite * 
+  ems:bool // extended-master-secret flag
+
+// For TLS 1.3, HS keeps the concrete ha and (optionally) aea, subject
+// to in Nego, and reminds them to KS as we progress in the
+// schedule. Both are also always bound as a function of the ghost
+// index.
+
+/// key-schedule states for TLS 1.2; will be split further. 
+type ks_client_state = 
+// | C_Init: 
+//    cr:random -> ks_client_state
+| C_12_Resume_CH: 
+    cr:random -> 
+    si:sessionInfo -> 
+    msId:TLSInfo.msId -> 
+    ms:ms -> ks_client_state
+//| C_12_Full_CH: 
+//    cr:random -> ks_client_state
+//
+// optional intermediate state within HS.client_ServerHelloDone 
+| C_12_wait_MS: 
+    csr:csRands -> 
+    alpha:ks_alpha12 -> 
+    id:TLSInfo.pmsId -> 
+    pms:pms -> ks_client_state
+//
+// state after HS.client_ServerHelloDone
+| C_12_has_MS: 
+    csr:csRands -> 
+    alpha:ks_alpha12 -> 
+    id:TLSInfo.msId -> 
+    ms:ms -> ks_client_state
+
+abstract type c13_wait_ServerHello 
+  (psks  : list (i:esId{~(no_psk i)})) 
+  (groups: list CommonDH.group) = 
+| C13_wait_ServerHello:
+  // symmetric extracts for the PSKs the client is proposing
+  // (the indexes are a function of those of the PKSs)
+  esl: list (i:esId{~(no_psk i)} & es i) ->
+  // private exponents for the honestly-generated shares the client is
+  // proposing (overwritten on hello_retry)
+  gxs: list CommonDH.dhi -> c13_wait_ServerHello psks groups
+
+// now just ams i:
+// abstract type c13_wait_ServerFinished (i: amsId) = 
+// abstract type c13_wait_ClientFinished (i: amsId) = 
+
+/// rekeying part of the final state, holding the *next* transport
+/// secret, separately for the client and the server.
+abstract type next_ts (i: ts_id) = secret (ts_of_ts i) 
+
+
+// intermediate state waiting for the the ...ServerHello digest
+abstract type s13_wait_ServerHello:
+| S13_wait_SH (i: esId) (idh): 
+    ha: kdfa {ha = ha_of_id i1} -> 
+    aea: option (aeAlg {aea = get_aeadAlg i1}) -> // still undefined when there is no PSK
+    cr:random -> 
+    sr:random -> 
+    es i ->
+    hs (ems_to hms i idh) -> ks_server_state
+
+abstract type s13_wait_ServerFinished (i: amsId) = 
+| S13_wait_ServerFinished (secret i)
+
+// to be similarly refactored 
+type ks_server_state =
+| S_Init: 
+    sr:random -> ks_server_state
+| S_12_wait_CKE_DH: 
+    csr:csRands -> 
+    alpha:ks_alpha12 -> 
+    our_share:(g:CommonDH.group & CommonDH.pre_keyshare g) -> ks_server_state
+| S_12_wait_CKE_RSA: 
+    csr: csRands -> 
+    alpha:ks_alpha12 -> ks_server_state
+| S_12_has_MS: 
+    csr:csRands -> 
+    alpha:ks_alpha12 -> 
+    id:TLSInfo.msId -> 
+    ms:ms -> ks_server_state
+| S_Done
+
+// Reflecting state separation from HS; still used for TLS 1.2
+type ks_state =
+| C: s:ks_client_state -> ks_state
+| S: s:ks_server_state -> ks_state
+
+// KeySchedule instances
+(*
+ * AR: changing state from rref to ref, with region captured in the refinement.
+ *)
+//type ks =
+//| KS: #region:rid -> state:(ref ks_state){HS.MkRef?.id state = region} -> ks
+//17-04-17 CF: expose it as a concrete ref?
+//17-04-17 CF: no need to keep the region, already in the ref.
+
+/// Extract keys and IVs from a derived TLS 1.3 traffic secret
+/// TODO
+/// 2-stage AEAD creation
+/// return abstract AEAD writer instance
+/// reader instance as a follow up call?
+/// key-install invariant
+/// regions?
+/// reader vs writer? 
+
+val derive_ae13:
+  #u: IK.usage -> // should be specific
+  #i: IK.id {IK.registered i} -> // should be refined
+  s: IK.secret u i -> 
+  info: IK.info {info = IK.get_info i} ->
+  parent: rgn -> 
+  ST (StreamAE.key (ae_traffic i))
+  (requires fun h0 -> True)
+  (ensures fun h0 k h1 -> True)
+
+let derive_ae13 #u #i s info parent = 
+  let k: AEAD.key (Derive i "key" Expand) = derive ha secret "key" Expand (parent, info.aea) in 
+  let iv: StreamAE.iv (Derive i "iv" Expand) = derive ha secret "iv" Expand (info.pv, info.aea) in
+  let w: StreamAE.writer i = StreamAE.wrapWriter k iv in 
+  w
+(* WAS:
+private let keygen_13 h secret ae : St (bytes * bytes) =
+  let kS = CoreCrypto.aeadKeySize ae in
+  let iS = CoreCrypto.aeadRealIVSize ae in
+  let kb = HKDF.hkdf_expand_label h secret "key" empty_bytes kS in
+  let ib = HKDF.hkdf_expand_label h secret "iv" empty_bytes iS in
+  (kb, ib)
+*)
+
+// // Extract finished keys
+// private let derive_finished13 h secret: St bytes =
+//   HKDF.hkdf_expand_label h secret "finished" empty_bytes (H.tagLen h)
+
+(* GONE: 
+// Create a fresh key schedule instance
+// We expect this to be called when the Handshake instance is created
+val create: #rid:rid -> role -> ST (ks * random)
+  (requires fun h -> rid<>root)
+  (ensures fun h0 (r,_) h1 ->
+    let KS #ks_region state = r in
+    stronger_fresh_region ks_region h0 h1
+    /\ extends ks_region rid
+    /\ modifies (Set.singleton rid) h0 h1
+    /\ modifies_rref rid (Set.singleton (Heap.addr_of (as_ref state))) (HS.HS?.h h0) (HS.HS?.h h1))
+
+let create #rid r =
+  ST.recall_region rid;
+  let ks_region = new_region rid in
+  let nonce = Nonce.mkHelloRandom r ks_region in
+  let istate = match r with
+    | Client -> C (C_Init nonce)
+    | Server -> S (S_Init nonce) in
+  (KS #ks_region (ralloc ks_region istate)), nonce
+*)
+
+private let group_of_valid_namedGroup
+  (g:valid_namedGroup)
+  : CommonDH.group
+  = Some?.v (CommonDH.group_of_namedGroup g)
+
+effect ST0 (a:Type) = ST a (fun _ -> True) (fun h0 _ h1 -> modifies_none h0 h1)
+
+val map_ST: ('a -> ST0 'b) -> list 'a -> ST0 (list 'b)
+let rec map_ST f x = match x with
+  | [] -> []
+  | a::tl -> f a :: map_ST f tl
+
+private let group_of_cks = function
+  | CommonDH.Share g _ -> Some?.v (CommonDH.namedGroup_of_group g)
+  | CommonDH.UnknownShare g _ -> g
+
+// 17-12-02 should call IK.initI, at least for TLS 1.3
+private let keygen (g:CommonDH.group)
+  : St (g:CommonDH.group & CommonDH.pre_keyshare g)
+  = (| g, CommonDH.keygen g |)
+
+assume val ks_client_init: ogl: option (list valid_namedGroup)
+  -> ST (option CommonDH.clientKeyShare)
+  (requires fun h0 -> True)
+  (ensures fun h0 ogxl h1 ->
+    (None? ogl ==> None? ogxl) /\
+    (Some? ogl ==> (Some? ogxl /\ Some?.v ogl == List.Tot.map group_of_cks (Some?.v ogxl))) /\
+    modifies_none h0 h1)
+
+(* 17-12-02 FIXME
+let ks_client_init ogl =
+  dbg ("ks_client_init "^(if ogl=None then "1.2" else "1.3"));
+  match ogl with
+  | None -> None // TLS 1.2
+  | Some gl ->   // TLS 1.3
+    let groups = List.Tot.map group_of_valid_namedGroup gl in
+    let gs = map_ST keygen groups in
+    let serialize_share (gx: CommonDH.dhi) =
+      let (| g, gx |) = gx in
+      match CommonDH.namedGroup_of_group g with
+      | None -> None // Impossible
+      | Some ng -> Some (CommonDH.Share g (CommonDH.pubshare #g gx)) in
+    let gxl = List.Tot.choose serialize_share gs in
+    // st := C (C_13_wait_SH cr [] gs);
+    Some gxl
+*)
+
+
+(* 17-11-25 functionally replacing the two functions below *)
+
+// the digest comes with its logical payload, ready to be MACed.
+// we will need a full spec of the early index. 
+// we can re-use this code at the server, except that we verify instead of MACing
+
+
+let binder_of_esid_id (i: esId{~(dummy i)}) = 
+  Binder i ExtBinder
+  // will be Derive (Derive i ...) ...
+
+val compute_es_and_bfk:
+  #rid: rgn -> 
+  (pskid:PSK.pskid * PSK.obfuscated_ticket_age) -> 
+  ST (i:esId{~(dummy i)} & es i * binderKey (binder_of_esid_id i) * IK.info (*TBC*) )
+  (requires fun h0 -> True)
+  (ensures fun h0 _ h1 -> modifies_none h0 h1)
+
+let compute_es_and_bfk #rid (pskid,_) =
+  // 17-11-25 rediscuss this callback
+  let i, pski, psk = read_psk pskid in
+  let ha = pski.early_hash in
+  dbg ("Loaded pre-shared key "^print_bytes pskid^": "^print_bytes psk);
+
+  let es: es i = magic() in // extract0 psk ha in
+  dbg ("Early secret: "^print_bytes es);
+
+  // // strange twist on usage; does it help re: salt collisions?
+  //
+  // let binder_key = 
+  //   if ApplicationPSK? i 
+  //   then derive_secret "ext binder" es ha 
+  //   else derive_secret "res binder" es ha
+  let lb = 
+    if ApplicationPSK? i //17-11-26 we need to know at run-time
+    then "ext binder" 
+    else "res binder" in
+
+  let bk: binderKey (binder_of_esid_id i) = magic() in 
+  let es_info = magic() in
+  (*
+  let bId = Binder i ll in
+  let bk: secret bId = magic() in // KDF.derive_secret ha es lb (H.emptyHash ha) in
+  dbg ("binder key["^lb^"]: "^print_bytes bk);
+
+  let bkfId = binderKey bId in 
+  let bfk: HMAC.UFCMA.key bkfId = KDF.derive bk ha "finished" in
+  dbg ("binder Finished key: "^print_bytes bfk);
+  *)
+  (| i, (es, bk, es_info) |)
+
+(* WAS:
+private let mk_binder (#rid) (pskid:PSK.pskid)
+  : ST ((i:binderId & bk:binderKey i) * (i:esId{~(dummy i)} & es i))
+  (requires fun h0 -> True)
+  (ensures fun h0 _ h1 -> modifies_none h0 h1)
+  =
+  let i, pski, psk = read_psk pskid in
+  let h = pski.early_hash in
+  dbg ("Loaded pre-shared key "^(print_bytes pskid)^": "^(print_bytes psk));
+  let es : es i = HKDF.extract #h (H.zeroHash h) psk in
+  dbg ("Early secret: "^(print_bytes es));
+  let ll, lb =
+    if ApplicationPSK? i then ExtBinder, "ext binder"
+    else ResBinder, "res binder" in
+  let bId = Binder i ll in
+  let bk = magic() in // HKDF.derive_secret h es lb (H.emptyHash h) in
+  dbg ("Binder key["^lb^"]: "^(print_bytes bk));
+  let bk = derive_finished13 h bk in
+  dbg ("Binder Finished key: "^(print_bytes bk));
+  let bk : binderKey bId = magic() in //HMAC.UFCMA.coerce (HMAC.UFCMA.HMAC_Binder bId) (fun _ -> True) rid bk in
+  (| bId, bk|), (| i, es |)
+
+let ks_client_13_get_binder_keys ks pskl =
+  let KS #rid st = ks in
+  let C (C_13_wait_SH cr [] gs) = !st in
+  let pskl = map_ST (mk_binder #rid) pskl in
+  let (bkl, esl) = List.Tot.split pskl in
+  st := C (C_13_wait_SH cr esl gs);
+  bkl
+*)
+
+// 17-11-25 new state-passing variant; why do we resample? impact on
+// the KS proof? We suppose Nego does the filtering. 
+
+let client13_HelloRetryRequest (g:CommonDH.group): ST0 (CommonDH.ikeyshare g) =
+  // TODO: just call initI g 
+  admit()
+//let x: CommonDH.ikeyshare g = CommonDH.keygen g in
+//let gX = CommonDH.pubshare #g s in
+//[(| g, x|)], gX
+
+(*
+let ks_client_13_hello_retry ks (g:CommonDH.group)
+  : ST0 (CommonDH.ikeyshare g) =
+  let KS #rid st = ks in
+  let C (C_13_wait_SH cr esl gs) = !st in
+  let s : CommonDH.keyshare g = CommonDH.keygen g in
+  st := C (C_13_wait_SH cr esl [(| g, s |)]);
+  CommonDH.pubshare #g s
+*)
+
+
+/// When 0-RTT is offered, derive the early data key and exporter
+/// secret from the early secret of the first offered PSK.
+
+let client13_0RTT 
+  (i: emsi) 
+  (es: secret i) //TODO does the secret embed its info? otherwise [ha,aea] required
+  (truncated_ClientHello: transcript) // ghost
+  (digest: Hashing.Spec.anyTag) // to be refined
+  (writer_parent: rgn) 
+  : ST (
+    secret (x0s_of_ems i truncated_ClientHello) * 
+    StreamAE.writer (ets_of_ems i truncated_ClientHello))
+  (requires fun h0 -> True 
+    // freshness of this transcript (from freshness of its nonce)
+    )
+  (ensures fun h0 r h1 ->
+    modifies_none h0 h1 
+    // except for the keys we derive
+    )
+  =
+  dbg ("client13_0RTT log="^print_bytes digest);
+  let ha = esId_hash i in
+  let aea = esId_ae i in
+  let info = (ha,aea) in
+
+  let x0si = x0s_of_ems i transcript in 
+  let x0s: secret x0si = derive es ha "e exp master" transcript digest info in
+  dbg ("Early exporter master secret:    "^print_bytes (leak_secret x0s));
+
+  let etsi = ets_of_ems i transcript in
+  let ets: secret etsi = derive es ha "c e traffic" transcript digest info in
+  dbg ("Client early traffic secret:     "^print_bytes (leak_secret ets));
+
+  let key0 = derive_streamAE #etsi ets Writer writer_parent in 
+  x0s, key0
+
+(* WAS: 
+let ks_client_13_ch ks (log:bytes): ST (exportKey * recordInstance)
+  (requires fun h0 ->
+    let kss = sel h0 (KS?.state ks) in
+    C? kss /\ C_13_wait_SH? (C?.s kss))
+  (ensures fun h0 r h1 ->
+    let KS #rid st = ks in
+    modifies_none h0 h1)
+  =
+  dbg ("ks_client_13_ch log="^(print_bytes log));
+  let KS #rid st = ks in
+  let C (C_13_wait_SH cr ((| i, es |) :: _) gs) = !st in
+
+  let h = esId_hash i in
+  let ae = esId_ae i in
+
+  let li = LogInfo_CH0 ({
+   li_ch0_cr = cr;
+   li_ch0_ed_ae = ae;
+   li_ch0_ed_hash = h;
+   li_ch0_ed_psk = empty_bytes; }) in
+
+  let log : hashed_log li = log in
+  let expandId : expandId li = ExpandedSecret (EarlySecretID i) ClientEarlyTrafficSecret log in
+  let ets = HKDF.derive_secret h es "c e traffic" log in
+  dbg ("Client early traffic secret:     "^print_bytes ets);
+  let expId : exportId li = EarlyExportID i log in
+  let early_export : ems expId = HKDF.derive_secret h es "e exp master" log in
+  dbg ("Early exporter master secret:    "^print_bytes early_export);
+  let exporter0 = (| li, expId, early_export |) in
+
+  // Expand all keys from the derived early secret
+  let (ck, civ) = keygen_13 h ets ae in
+  dbg ("Client 0-RTT key:                "^print_bytes ck^", IV="^print_bytes civ);
+
+  let id = ID13 (KeyID expandId) in
+  let ckv: StreamAE.key id = ck in
+  let civ: StreamAE.iv id  = civ in
+  let rw = StAE.coerce HyperHeap.root id (ckv @| civ) in
+  let r = StAE.genReader HyperHeap.root rw in
+  let early_d = StAEInstance r rw in
+  exporter0, early_d
+*)
+
+
+val server12_init_dh: ks:ks -> cr:random -> pv:protocolVersion -> cs:cipherSuite -> ems:bool -> g:CommonDH.group -> ST (CommonDH.share g)
+  (requires fun h0 ->
+    let kss = sel h0 (KS?.state ks) in
+    S? kss /\ S_Init? (S?.s kss)
+    /\ CipherSuite? cs
+    /\ (let CipherSuite kex _ _ = cs in
+         (kex = Kex_DHE \/ kex = Kex_ECDHE)))
+  (ensures fun h0 r h1 ->
+    let KS #rid st = ks in
+    modifies (Set.singleton rid) h0 h1
+    /\ modifies_rref rid (Set.singleton (Heap.addr_of (as_ref st))) (HS.HS?.h h0) (HS.HS?.h h1))
+
+let server12_init_dh ks cr pv cs ems g =
+  dbg "server12_init_dh";
+  let KS #region st = ks in
+  let S (S_Init sr) = !st in
+  let CipherSuite kex sa ae = cs in
+  let our_share = CommonDH.keygen g in
+  let _ = print_share (CommonDH.pubshare our_share) in
+  let csr = cr @| sr in
+  st := S (S_12_wait_CKE_DH csr (pv, cs, ems) (| g, our_share |));
+  CommonDH.pubshare our_share
+
+
+/// Once TLS 1.3 is accepted, compute all keys up to the handshake
+/// secret (except for now for the optional [server13_0rtt_key],
+/// which further require the client transcript).
+///
+val server13_init:
+  cr: random ->
+  sr: random
+  cs: cipherSuite ->
+  pskid: option PSK.pskid ->
+  g_gx: option (g:CommonDH.group & CommonDH.share g) ->
+  ST (
+    i: esId (* TODO: carefully relate i to pskid *) &
+    
+    option CommonDH.serverKeyShare * 
+    option (binderKey (fnk_of_ts (ets_of_ems i))))
+  (requires fun h0 -> 
+    // stateless conditions: 
+    (Some? g_gx \/ Some? pskid) /\
+    (Some? g_gx ==> Some? (CommonDH.namedGroup_of_group (dfst (Some?.v g_gx)))) /\
+    CipherSuite13? cs
+    // will also require the global keyed invariant
+    )
+  (ensures fun h0 (gy, bk) h1 ->
+    // will modify the global keyed footprint and restore its invariant;
+    // any more details required? 
+    modifies_none h0 h1 /\
+    (Some? bk <==> Some? pskid) /\
+    (Some? gy \/ Some? bk) )
+
+let server13_init cr sr cs pskid g_gx =
+  dbg "server13_init";
+  let CipherSuite13 aea ha = cs in
+
+  // retrieve optional pre-shared key; should the index be pski instead?
+  let (| i, psk0, ha |): ( i:esId & psk i & ha: Hashing.Spec.alg {ha = ha_of_id i} ) =
+    match pskid with 
+    | None ->
+      dbg "No PSK selected.";
+      (| i, psk_dummy ha, ha |) 
+    | Some id -> 
+      dbg ("Using negotiated PSK identity: "^print_bytes id);
+        //17-11-26 should this branch move to PSK? 
+        match Ticket.check_ticket id with
+        | Some (Ticket.Ticket13 cs li rmsId rms) ->
+          dbg ("Ticket RMS: "^print_bytes rms);
+          let i = ResumptionPSK #li rmsId in
+          let CipherSuite13 _ ha = cs in //17-11-26 no consistency check? 
+          let nonce, _ = split id 12 in  //17-11-26 what's this nonce? 
+          let psk0 = KDF.derive_secret ha rms "resumption" nonce in
+          (i, psk, ha)
+        | None ->
+          let i, pski, psk = read_psk id in //17-11-26 no consistency check?
+          (i, psk, pski.early_hash) in
+  if Some? pskid then dbg ("Pre-shared key: "^leak_psk psk);
+
+  // extract early master secret
+  let i0 = ems_of_psk i in 
+  let es: secret i0 = extract0 psk0 ha in 
+  dbg ("Computed early secret:           "^leak_secret es);
+  let bfko =
+    match pskid with 
+    | None -> None
+    | Some _ -> // optionally compute the binder-verification key
+      let lbl = binder_label i in
+      let bnsi = bns_of_ems i0 in
+      let bns: secret bnsi = derive es ha lbl Expand info in
+      let bfkId = binderKey i in
+      let info0 = magic() in // missing region and logical payload
+      let bfk: HMAC.UFCMA.key i = derive bns ha "finished" Expand info0 in
+      dbg ("binder key:                      "^print_bytes bk);
+      dbg ("binder Finished key:             "^print_bytes bk);
+      Some bfk
+
+  // TODO optionally compute the 0RTT key too? 
+
+  // extract handshake secret, mixing-in the optional DH secret. 
+  let salt1: salt (salt_of_ms i0) = derive es ha "derived" Expand () in
+  let idh, hs =
+    match g_gx with
+    | None -> 
+        let hs = extractP ha salt1 in
+        NoIDH, hs
+    | Some (| g, gX |) ->
+        let gY, hs = extractR ha g gX in 
+        IDH gX gY, hs in
+  dbg ("Handshake salt:                  "^print_bytes salt);
+  dbg ("Handshake secret:                "^print_bytes hs);
+  gY, bfko, (*local state:*) hs 
+
+(* WAS:
+let ks_server_13_init ks cr cs pskid g_gx =
+  dbg ("ks_server_init");
+  let KS #region st = ks in
+  let S (S_Init sr) = !st in
+  let CipherSuite13 ae h = cs in
+  let esId, es, bk =
+    match pskid with
+    | Some id ->
+      dbg ("Using negotiated PSK identity: "^(print_bytes id));
+      let i, psk, h : esId * bytes * Hashing.Spec.alg =
+        match Ticket.check_ticket id with
+        | Some (Ticket.Ticket13 cs li rmsId rms) ->
+          dbg ("Ticket RMS: "^(print_bytes rms));
+          let i = ResumptionPSK #li rmsId in
+          let CipherSuite13 _ h = cs in
+          let nonce, _ = split id 12 in
+          let psk = HKDF.derive_secret h rms "resumption" nonce in
+          (i, psk, h)
+        | None ->
+          let i, pski, psk = read_psk id in
+          (i, psk, pski.early_hash)
+        in
+      dbg ("Pre-shared key: "^(print_bytes psk));
+      let es = HKDF.hkdf_extract h (H.zeroHash h) psk in
+      let ll, lb =
+        if ApplicationPSK? i then ExtBinder, "ext binder"
+        else ResBinder, "res binder" in
+      let bId = Binder i ll in
+      let bk = HKDF.derive_secret h es lb (H.emptyHash h) in
+      let bk = finished_13 h bk in
+      dbg ("binder key:                      "^print_bytes bk);
+      dbg ("binder Finished key:             "^print_bytes bk);
+      let bk : binderKey bId = HMAC.UFCMA.coerce (HMAC.UFCMA.HMAC_Binder bId) (fun _ -> True) region bk in
+      i, es, Some (| bId, bk |)
+    | None ->
+      dbg "No PSK selected.";
+      let esId = NoPSK h in
+      let es : es esId = HKDF.hkdf_extract h (H.zeroHash h) (H.zeroHash h) in
+      esId, es, None
+    in
+  dbg ("Computed early secret:           "^print_bytes es);
+  let saltId = Salt (EarlySecretID esId) in
+  let salt = HKDF.derive_secret h es "derived" (H.emptyHash h) in
+  dbg ("Handshake salt:                  "^print_bytes salt);
+  let gy, hsId, hs =
+    match g_gx with
+    | Some (| g, gx |) ->
+      let gy, gxy = CommonDH.dh_responder gx in
+      dbg ("DH shared secret: "^(print_bytes gxy));
+      let hsId = HSID_DHE saltId g gx gy in
+      let hs : hs hsId = HKDF.hkdf_extract h salt gxy in
+      Some (CommonDH.Share g gy), hsId, hs
+    | None ->
+      let hsId = HSID_PSK saltId in
+      let hs : hs hsId = HKDF.hkdf_extract h salt (H.zeroHash h) in
+      None, hsId, hs
+    in
+  dbg ("Handshake secret:                "^print_bytes hs);
+  st := S (S_13_wait_SH (ae, h) cr sr (| esId, es |) (| hsId, hs |));
+  gy, bk
+*)
+
+let server13_0RTT 
+  (i: esId) 
+  (idh:_) 
+  (ks: s13_wait_ServerHello i idh) 
+  (truncated_ClientHello: transcript)
+  (digest: Hashing.Spec.anyTag) 
+  (reader_parent: rgn):
+  ST (
+    secret (x0s_of_ems i transcript_ClientHello) * 
+    StreamAE.reader (ets_of_ems i transcript_ClientHello))
+  (requires fun h0 -> True)
+  (ensures fun h0 _ h1 -> modifies_none h0 h1)
+=
+  dbg "server13_0rtt_key";
+  let S13_wait_ServerHello ha aea _ _ es _ = ks in 
+  let info = (ha, aea) in
+
+  let x0si = x0s_of_ems i transcript_ClientHello in
+  let x0s = secret x0si = derive es ha "e exp master" truncated_ClientHello digest info in
+  dbg ("Early exporter master secret:    "^leak_secret x0s);
+
+  let ets = derive es ha "c e traffic" truncated_ClientHello digest info in
+  dbg ("Client early traffic secret:     "^leak_secret ets);
+
+  let key0 = derive_streamAE #etsi ets Reader reader_parent in
+  (x0s, key0)
+
+/// Continues from the handshake secret, now that we have the handshake
+/// digest up to ServerHello. We stop at the application master secret
+/// and return the handshake AE keys to install and the Finished keys.
+
+val server13_ServerHello: 
+  i: esId ->
+  idh:_ ->
+  ks: s13_wait_ServerHello i idh ->
+  tr: transcript ->
+  digest: Hashing.Spec.anyTag ->
+  ST (
+    i: hsid {i = hms_of_ems i idh} &
+    s13_wait_ServerFinished (ams_of_hms i) *
+    StreamAE.reader (cts_of_hms i) *
+    StreamAE.writer (sts_of_hms i) * 
+
+    )
+  (requires fun h0 -> True)
+  (ensures fun h0 r h1 -> modifies_none h0 h1)
+
+let server13_ServerHello ks log =
+  dbg ("server13_ServerHello, hashed log = "^print_bytes digest);
+
+  let S13_wait_ServerHello ha aea _ _ es hs = ks in
+  // Derived handshake traffic secrets and keys 
+  let cts = derive ha hs "c hs traffic" log info in
+  let sts = derive ha hs "s hs traffic" log info in 
+
+  // Handshake traffic keys
+  let w = derive_streamAE sts info Writer writer_parent in 
+  let r = derive_streamAE cts info Reader reader_parent in 
+
+  // Finished keys (hiding too much their regions and logical payloads)
+  let cfk1 = finished_13 h cts in
+  let sfk1 = finished_13 h sts in
+
+  dbg ("handshake traffic secret[C]:     "^sprint_secret cts);
+  dbg ("handshake traffic secret[S]:     "^sprint_secret sts);
+  dbg ("finished key[C]:                 "^sprint_secret cfk1);
+  dbg ("finished key[S]:                 "^sprint_secret sfk1);
+  //dbg ("handshake key[C]:                "^print_bytes ck^", IV="^print_bytes civ);
+  //dbg ("handshake key[S]:                "^print_bytes sk^", IV="^print_bytes siv);
+
+  let saltId = Salt (HandshakeSecretID hsId) in
+  let salt = derive_secret hs ha "derived" Expand in
+  //dbg ("Application salt:                "^print_bytes salt);
+  let amsi = ams_of_hms hmsi in
+  let ams: secret amsi = extract2 salt ha in
+  dbg ("Application secret:              "^sprint_secret ams);
+
+  let next = S13_wait_ServerFinished #amsi ha aea ams in
+  (| hmsi, (next, r, w) |)
+
+
+// Will become private; public API will have
+// client12_keygen: ks -> (i:id * w:StatefulLHAE.writer i)
+// server12_keygen: ...
+val ks_12_finished_key: st: ks_state -> ST (key:TLSPRF.key)
+  (requires fun h0 ->
+    match st with
+    | C (C_12_has_MS _ _ _ _) | S (S_12_has_MS _ _ _ _) -> True
+    | _ -> False)
+  (ensures fun h0 r h1 -> modifies Set.empty h0 h1)
+
+let ks_12_finished_key st =
+  let ms = match st with
+  | C (C_12_has_MS _ _ _ ms) -> ms
+  | S (S_12_has_MS _ _ _ ms) -> ms in
+  TLSPRF.coerce ms
+
+let ks_12_ms st = 
+  match st with 
+  | C (C_12_has_MS _ _ msId ms) -> (msId, ms)
+  | S (S_12_has_MS _ _ msId ms) -> (msId, ms)
+
+private val ks_12_record_key: st: ks_state -> St recordInstance
+let ks_12_record_key st =
+  dbg "ks_12_record_key";
+  let role, csr, alpha, msId, ms =
+    match st with
+    | C (C_12_has_MS csr alpha msId ms) -> Client, csr, alpha, msId, ms
+    | S (S_12_has_MS csr alpha msId ms) -> Server, csr, alpha, msId, ms in
+  let cr, sr = split csr 32 in
+  let (pv, cs, ems) = alpha in
+  let kdf = kdfAlg pv cs in
+  let ae = get_aeAlg cs in
+  let id = ID12 pv msId kdf ae cr sr role in
+  let AEAD alg _ = ae in (* 16-10-18 FIXME! only correct for AEAD *)
+  let klen = CoreCrypto.aeadKeySize alg in
+  let slen = AEADProvider.salt_length id in
+  let expand = TLSPRF.kdf kdf ms (sr @| cr) (klen + klen + slen + slen) in
+  dbg ("keystring (CK, CIV, SK, SIV) = "^print_bytes expand);
+  let k1, expand = split expand klen in
+  let k2, expand = split expand klen in
+  let iv1, iv2 = split expand slen in
+  let wk, wiv, rk, riv =
+    match role with
+    | Client -> k1, iv1, k2, iv2
+    | Server -> k2, iv2, k1, iv1 in
+  let w = StAE.coerce HyperHeap.root id (wk @| wiv) in
+  let rw = StAE.coerce HyperHeap.root id (rk @| riv) in
+  let r = StAE.genReader HyperHeap.root rw in
+  StAEInstance r w
+
+(* 1.2 resumption *)
+
+// We can potentially 1.2 resume from 1.2 or 1.3 ClientHello
+let client12_resume (ks:ks) (sr:random) (pv:protocolVersion) (cs:cipherSuite)
+  (ems:bool) (msId:TLSInfo.msId) (ms:bytes) : ST recordInstance
+  (requires fun h0 ->
+    let kss = sel h0 (KS?.state ks) in
+    C? kss /\ (C_12_Full_CH? (C?.s kss) \/ C_13_wait_SH? (C?.s kss)))
+  (ensures fun h0 r h1 ->
+    let KS #rid st = ks in
+    modifies (Set.singleton rid) h0 h1
+    /\ modifies_rref rid (Set.singleton (Heap.addr_of (as_ref st))) (HS.HS?.h h0) (HS.HS?.h h1))
+  =
+  dbg "client12_resume";
+  let KS #rid st = ks in
+  let cr = match !st with
+    | C (C_12_Full_CH cr) -> cr
+    | C (C_13_wait_SH cr _ _) -> cr in
+  dbg ("Recall MS: "^print_bytes ms);
+  st := C (C_12_has_MS (cr @| sr) (pv, cs, ems) msId ms);
+  ks_12_record_key ks
+
+let server12_resume (ks:ks) (cr:random) (pv:protocolVersion) (cs:cipherSuite)
+  (ems:bool) (msId:msId) (ms:bytes) =
+  dbg ("server12_resume");
+  let KS #region st = ks in
+  let S (S_Init sr) = !st in
+  dbg ("Recall MS: "^print_bytes ms);
+  st := S (S_12_has_MS (cr @| sr) (pv, cs, ems) msId ms);
+  ks_12_record_key ks
+
+(******************************************************************)
+
+// log is the raw HS log, used for EMS derivation
+val server12_cke_dh: ks:ks -> gy:(g:CommonDH.group & CommonDH.share g) ->
+  log:bytes -> ST (recordInstance)
+  (requires fun h0 ->
+    let kss = sel h0 (KS?.state ks) in
+    S? kss /\ S_12_wait_CKE_DH? (S?.s kss) /\
+    (let S (S_12_wait_CKE_DH _ _ (| g', _ |)) = kss in
+    g' = dfst gy)) // Responder share must be over the same group as initiator's
+  (ensures fun h0 r h1 ->
+    let KS #rid st = ks in
+    modifies (Set.singleton rid) h0 h1
+    /\ modifies_rref rid (Set.singleton (Heap.addr_of (as_ref st))) (HS.HS?.h h0) (HS.HS?.h h1))
+let server12_cke_dh ks gy hashed_log =
+  dbg "server12_cke_dh";
+  let KS #region st = ks in
+  let S (S_12_wait_CKE_DH csr alpha (| g, gx |)) = !st in
+  let (pv, cs, ems) = alpha in
+  let (| _, gy |) = gy in
+  let _ = print_share gy in
+  let pmsb = CommonDH.dh_initiator #g gx gy in
+  dbg ("PMS: "^print_bytes pmsb);
+  let pmsId = PMS.DHPMS g (CommonDH.pubshare gx) gy (PMS.ConcreteDHPMS pmsb) in
+  let kef = kefAlg pv cs ems in
+  let msId, ms =
+    if ems then
+      begin
+      let ms = TLSPRF.prf (pv,cs) pmsb (utf8 "extended master secret") hashed_log 48 in
+      dbg ("extended master secret:"^(print_bytes ms));
+      let msId = ExtendedMS pmsId hashed_log kef in
+      msId, ms
+      end
+    else
+      begin
+      let ms = TLSPRF.extract kef pmsb csr 48 in
+      dbg ("master secret:"^print_bytes ms);
+      let msId = StandardMS pmsId csr kef in
+      msId, ms
+      end
+    in
+  st := S (S_12_has_MS csr alpha msId ms);
+  ks_12_record_key ks
+
+(**
+// Called after receiving server hello; server accepts resumption proposal
+// This function only checks the agility paramaters compared to the resumed sessionInfo
+// and returns to the handshake whether the resumption is permissible
+val client12_resume: ks:ks -> random -> pv:protocolVersion -> cs:cipherSuite -> ST unit
+  (requires fun h0 ->
+    let kss = sel h0 (KS?.state ks) in
+    C? kss /\ C_12_Resume_CH? (C?.s kss))
+  (ensures fun h0 r h1 ->
+    let KS #rid st = ks in
+    modifies (Set.singleton rid) h0 h1
+    /\ modifies_rref rid (Set.singleton (Heap.addr_of (as_ref st))) (HS.HS?.h h0) (HS.HS?.h h1))
+
+let client12_resume ks sr pv cs =
+  let KS #region st = ks in
+  let C (C_12_Resume_CH cr si msId ms) = !st in
+  let csr = cr @| sr in
+  let ems = si.extended_ms in
+  st := C (C_12_has_MS csr (pv, cs, ems) msId ms)
+*)
+
+// The two functions below are similar but we decide not to factor them because:
+//   1. they use different arguments
+//   2. they use different return types
+//   3. they are called at different locations
+
+val client13_ServerHello:
+  psks: list (i:esId{~(no_psk i)}) -> groups: list CommonDH.group -> // ghosts indexing ks
+  ks: c13_wait_ServerHello psks groups -> 
+  sr: random -> 
+  cs: cipherSuite -> 
+  transcript: bytes ->
+  accepted_psk: option (n:nat{n < length psks}) -> 
+  accepted_group: CommonDH.group {List.mem g groups} -> 
+  gy: CommonDH.share g -> 
+  ST ( 
+    i: hsId {i = hsId_of_es i) & // next caller index, for convenience
+    (*ks':*) c13_wait_finished1 (amsId_of_hs i) *
+    (*cfk:*) MAC.UFCMA.key (cfkId_of_hs i transcript) *
+    (*sfk:*) MAC.UFCMA.key (sfkId_of_hs i transcript) *
+    (*hsw:*) StreamAE.writer (ctsId_of_hs i) *
+    (*hsr:*) StreamAE.reader (stsID_of_hs i) )
+  (requires fun h0 -> True)
+  (ensures fun h0 r h1 -> modifies_none h0 h1)
+
+let client13_ServerHello psks groups ks sr cs log accept_psk g gy =
+  dbg ("ks_client_13_sh hashed_log = "^print_bytes log);
+  let C13_wait_ServerHello esl gxs = ks in
+  let Some gx = List.Tot.find (
+      fun ((| g', _ |):(x:CommonDH.group & CommonDH.keyshare g)) -> g = g'
+    ) gc in
+  let (| g, gx |) = gx in
+  let b = print_share gy in
+  let gxy = CommonDH.dh_initiator #g gx gy in
+  dbg ("DH shared secret: "^print_bytes gxy);
+  let CipherSuite13 ae h = cs in
+  let gx = CommonDH.pubshare gx in
+
+  // Early secret: must derive zero here as hash is not known before
+  let esId, es =
+    match esl, accept_psk with
+    | l, Some n ->
+      let Some (| i, es |) : option (i:esId & es i) = List.Tot.nth l n in
+      dbg ("recallPSK early secret:          "^print_bytes es);
+      i, es
+    | _, None ->
+      let es = HKDF.hkdf_extract h (H.zeroHash h) (H.zeroHash h) in
+      dbg ("no PSK negotiated. Early secret: "^print_bytes (leak_secret es));
+      NoPSK h, es in
+
+  let saltId = Salt (EarlySecretID esId) in
+  let salt = HKDF.derive_secret h es "derived" (H.emptyHash h) in
+  dbg ("handshake salt:                  "^print_bytes (leak_salt salt));
+
+  let hsId = HSID_DHE saltId g gx gy in
+  let hs : hs hsId = HKDF.hkdf_extract h salt gxy in
+  dbg ("handshake secret:                "^print_bytes (leak_secret hs));
+
+  let secretId = HandshakeSecretID hsId in
+  let li = LogInfo_SH ({
+    li_sh_cr = cr;
+    li_sh_sr = sr;
+    li_sh_ae = ae;
+    li_sh_hash = h;
+    li_sh_psk = None;
+  }) in
+  let log: hashed_log li = log in
+  let c_expandId = ExpandedSecret secretId ClientHandshakeTrafficSecret log in
+  let s_expandId = ExpandedSecret secretId ServerHandshakeTrafficSecret log in
+
+  let cts = HKDF.derive_secret h hs "c hs traffic" log in
+  let sts = HKDF.derive_secret h hs "s hs traffic" log in
+  let (ck,civ) = keygen_13 h cts ae in
+  let (sk,siv) = keygen_13 h sts ae in
+  dbg ("handshake traffic secret[C]:     "^print_bytes cts);
+  dbg ("handshake traffic secret[S]:     "^print_bytes sts);
+  dbg ("handshake key[C]:                "^print_bytes ck^", IV="^print_bytes civ);
+  dbg ("handshake key[S]:                "^print_bytes sk^", IV="^print_bytes siv);
+
+  // Finished keys
+  let cfkId = FinishedID c_expandId in
+  let sfkId = FinishedID s_expandId in
+  let cfk1 = finished_13 h cts in
+  dbg ("finished key[C]: "^(print_bytes cfk1));
+  let sfk1 = finished_13 h sts in
+  dbg ("finished key[S]: "^(print_bytes sfk1));
+
+  let cfk1 : fink cfkId = HMAC.UFCMA.coerce (HMAC.UFCMA.HMAC_Finished cfkId) (fun _ -> True) region cfk1 in
+  let sfk1 : fink sfkId = HMAC.UFCMA.coerce (HMAC.UFCMA.HMAC_Finished sfkId) (fun _ -> True) region sfk1 in
+
+  (*TODO factor out *)
+  let id = ID13 (KeyID c_expandId) in
+  assert_norm(ID13 (KeyID s_expandId) = peerId id);
+  let ckv: StreamAE.key id = ck in
+  let civ: StreamAE.iv id  = civ in
+  let skv: StreamAE.key (peerId id) = sk in
+  let siv: StreamAE.iv (peerId id)  = siv in
+  let w = StAE.coerce HyperHeap.root id (ckv @| civ) in
+  let rw = StAE.coerce HyperHeap.root id (skv @| siv) in
+  let r = StAE.genReader HyperHeap.root rw in
+
+  let saltId = Salt (HandshakeSecretID hsId) in
+  let salt = HKDF.derive_secret h hs "derived" (H.emptyHash h) in
+  let asId = ASID saltId in
+  let ams: ams asId = HKDF.hkdf_extract h salt (H.zeroHash h) in
+  dbg ("application salt:                "^print_bytes (leak_salt salt));
+  dbg ("application secret:              "^print_bytes (leak_secret ams));
+
+  let next = C13_wait_ServerFinished ae h ams in
+  (next, cfk1, sfk1, hs_wr, hs_rd)
+
+(******************************************************************)
+
+let client13_ServerFinished
+  (i: amsId) 
+  (state: c13_wait_Finished1 i) // including [transcript1]
+  (transcript2: transcript): 
+  ST (
+    c13_wait_Finished2 i * 
+    MAC.UFCMA.key (cfkId_of_hs i transcript1) *
+    MAC.UFCMA.key (sfkId_of_hs i transcript1) *
+    StreamAE.reader (askId_of_hs i transcript2) *
+    StreamAE.writer (ackId_of_hs i transcript2)
+    exporter (ex1Id_of_hs i transcript2) )
+    
+  (requires fun h0 -> True)
+  (ensures fun h0 r h1 -> modifies_none h0 h1 (*TBC*) )
+=
+  dbg ("ks_client_13_sf hashed_log = "^print_bytes transcript1);
+  let C13_wait_Finished1 h ae transcript_fk cfk sfk ams = state in
+
+  // let FinishedID #li _ = dfst cfk in // TODO loginfo
+  // let secretId = ApplicationSecretID asId in
+  // let c_expandId = ExpandedSecret secretId ClientApplicationTrafficSecret log in
+  // let s_expandId = ExpandedSecret secretId ClientApplicationTrafficSecret log in
+  // let emsId : exportId li = ExportID asId log in
+
+  let i2 = amdId_of_hs i in 
+  let ctsId = ctsId_of_as i2 transcript2 in 
+  let stsId = ctsId_of_as i2 transcript2 in 
+  let exsId = exsId_of_as i2 transcript2 in 
+
+  let info = magic() in 
+  let cts: secret ctsId = IK.derive h ams "c ap traffic" transcript2 info in
+  let sts: secret stsId = IK.derive h ams "s ap traffic" transcript2 info in
+  let exs: secret exsId = IK.derive h ams "exp master"   transcript2 info in
+  let (ck,civ) = keygen_13 h cts ae in
+  let (sk,siv) = keygen_13 h sts ae in
+  dbg ("application traffic secret[C]:   "^print_bytes cts);
+  dbg ("application traffic secret[S]:   "^print_bytes sts);
+  dbg ("exporter master secret:          "^print_bytes ems);
+  dbg ("application key[C]:              "^print_bytes ck^", IV="^print_bytes civ);
+  dbg ("application key[S]:              "^print_bytes sk^", IV="^print_bytes siv);
+
+  let id = ID13 (KeyID c_expandId) in
+  assert_norm(peerId id = ID13 (KeyID s_expandId));
+  let ckv: StreamAE.key id = ck in
+  let civ: StreamAE.iv id  = civ in
+  let w = StAE.coerce HyperHeap.root id (ckv @| civ) in
+  let skv: StreamAE.key (peerId id) = sk in
+  let siv: StreamAE.iv (peerId id)  = siv in
+  let rw = StAE.coerce HyperHeap.root id (skv @| siv) in
+  let r = StAE.genReader HyperHeap.root rw in
+
+  let next = C13_wait_Finished2 h ae ams (cts,sts) in
+  (next, cfk, sfk, r, w, exs)
+
+
+/// Continues from the application master secret, now that we have the
+/// digest of the complete handshake. We keep this secret (required to
+/// compute the RMS) and return the application AE keys to install. We
+/// also immediately derive and return the next transport secrets, to
+/// help with forward secrecy.
+/// 
+val server13_ServerFinished: 
+  #i: amsId -> 
+  s: ams i ->
+  ha: kdfa {ha = ha_of_id i} -> 
+  aea: option (aeAlg {aea = get_aeadAlg i}) -> 
+  tr: transcript -> 
+  tag: digest i tr -> 
+  ST (
+    StreamAE.reader (cts_of_ams i) * 
+    StreamAE.writer (sts_of_ams i) *
+    secret (x1s_of_ams i) *
+    next_ts (cts_of_ams i) *
+    next_ts (sts_of_ams i) )
+  (requires fun h0 -> True)
+  (ensures fun h0 r h1 -> True)
+
+let server13_ServerFinished #i ams ha aea tr tag =   
+  let ems = derive_secret ams h "exp master" tr tag in
+  let cts = derive ha ams "c ap traffic" tr tag ha in
+  let sts = derive ha ams "s ap traffic" tr tag ha in
+  let r   = derive_streamAE ha ae cts parent in
+  let w   = derive_streamAE ha ae sts parent in 
+  let cts'= derive ha cts "traffic upd" Expand ha in
+  let sts'= derive ha cts "traffic upd" Expand ha in 
+  dbg ("server13_ServerFinished hash   = "^print_bytes tag);
+  dbg ("exporter master secret:          "^print_bytes (leak_secret ems));
+  dbg ("application traffic secret[C,0]: "^print_bytes (leak_secret cts));
+  dbg ("application traffic secret[S,0]: "^print_bytes (leak_secret sts));
+  dbg ("application traffic secret[C,1]: "^print_bytes (leak_secret cts'));
+  dbg ("application traffic secret[S,1]: "^print_bytes (leak_secret sts'));
+  r, w, ems, cts', sts'
+
+/// Final step for both client13 and server13, returning the
+/// resumption master secret; the application master secret should
+/// then be discarded.
+
+val rms_of_ClientFinished: 
+  #i: amsId -> 
+  s: ams i -> 
+  ha: kdfa {ha = ha_of_id i} -> 
+  tr: transcript -> // [ClientHello; ...; ClientFinished]
+  tag: digest i tr -> 
+  ST (secret (rms_of_ams i tr))
+  (requires fun h0 -> True 
+    // multi-functionality inv
+    )
+  (ensures fun h0 r h1 -> True 
+    // multi-functionality inv
+    // modifies some KDF
+    )
+let server13_ClientFinished #i ams ha tr tag =
+  let rms = derive_secret ha ams "res master" tr tag ha in
+  dbg ("resumption master secret:        "^print_bytes (leak_secret rms));
+  rms
+
+/// For each ticket received from the server,
+/// generate a PSK from the current RMS and incoming ticket nonce
+/// (may be called several times).
+///
+/// Sharable between client13 and server13
+
+// problem: there is no transcript associated with nonce, so we will
+// probably need to add some ExpandNonce.
+
+val derive_resumption_secret:
+  i: id ->
+  s: secret i ->
+  ha: kdfa {ha = ha_of_id i} -> 
+  nonce: bytes -> // really?
+  : ST (secret (psk_of_rms i i))
+  (requires fun h0 -> True)
+  (ensures fun h0 r h1 -> modifies_none h0 h1)
+=
+  dbg "ks_client_13_rms";
+  dbg ("Recall RMS: "^hex_of_bytes rms);
+  derive ha rms "resumption" (ExpandLog nonce) ha 
+
+/// Rekeying for both client13 and server13, also returning the next
+/// transport secret.
+/// 
+let rekey 
+  (#i: ts_id) 
+  (ha: prfa {ha = ha_of_i i})
+  (aea: aeadAlg {aea = aeadAlg_of_i i}) 
+  (ts: next_transport_secret i) 
+  (rw: TLSConstants.rw {rw = rw_of_i i})
+  (parent: rgn): 
+  ST( 
+    StreamAE.key (ts_of_ts i) ) rw *
+    next_transport_secret (ts_of_ts i) 
+  (requires fun h0 -> True)
+  (ensures fun h0 r h1 -> True)
+=
+  let k  = derive_streamAE #i ts rw (aea,parent) in 
+  let j: ts_id = ts_of_ts i in 
+  let ts: secret j = derive ts ha "traffic upd" Expand in 
+  k, ts
+    
+
+(******************************************************************)
+
+// Called by Hanshake when DH key echange is negotiated; 
+// 3 incoming states: was (C_12_Full_CH? (C?.s st) \/ C_12_Resume_CH? (C?.s st) \/ C_13_wait_SH? (C?.s st)))
+
+val client12_full_dh: 
+  cr: random -> 
+  sr: random -> 
+  pv: protocolVersion ->
+  cs: cipherSuite -> 
+  ems: bool -> 
+  gx:(g:CommonDH.group & CommonDH.share g) -> ST (CommonDH.share (dfst gx))
+  (requires fun h0 -> True)
+  (ensures fun h0 r h1 ->
+    (C_12_wait_MS? st \/ C_12_has_MS? st) /\ 
+    modifies_none h0 h1 // TODO modifies for DH
+  )
+let client12_full_dh ks sr pv cs ems (|g,gx|) =
+  let KS #region st = ks in
+  let csr = cr @| sr in
+  let alpha = (pv, cs, ems) in
+  let gy, pmsb = CommonDH.dh_responder #g gx in
+  dbg (sprint_share gx);
+  dbg (sprint_share gy);
+  dbg ("PMS: "^print_bytes pmsb);
+  let dhpmsId = PMS.DHPMS g gx gy (PMS.ConcreteDHPMS pmsb) in
+  let ns =
+    if ems then
+      C_12_wait_MS csr alpha dhpmsId pmsb
+    else
+      let kef = kefAlg pv cs false in
+      let ms = TLSPRF.extract kef pmsb csr 48 in
+      dbg ("master secret: "^print_bytes ms);
+      let msId = StandardMS dhpmsId csr kef in
+      C_12_has_MS csr alpha msId ms in
+  ns, gy
+
+// Called by Handshake after server hello when a full RSA key exchange is negotiated
+// returns the encrypted (currently disabled)
+// pre was: (C_12_Full_CH? (C?.s st) \/ C_12_Resume_CH? (C?.s st)))
+val client12_full_rsa: 
+  cr: random -> 
+  sr:random -> 
+  pv:protocolVersion -> 
+  cs:cipherSuite -> 
+  ems:bool -> 
+  RSAKey.pk -> ST (ks_client_state * bytes)
+  (requires fun h0 -> True)
+  (ensures fun h0 (st,r) h1 -> 
+    (C_12_wait_MS? st \/ C_12_has_MS? st) /\ 
+    modifies_none h0 h1 // TODO modifies for RSA
+  )
+let client12_full_rsa cr sr pv cs ems pk =
+  let alpha = (pv, cs, ems) in
+  let csr = cr @| sr in
+  let rsapms = PMS.genRSA pk pv in
+  let pmsb = PMS.leakRSA pk pv rsapms in
+  let encrypted = CoreCrypto.rsa_encrypt (RSAKey.repr_of_rsapkey pk) CoreCrypto.Pad_PKCS1 pmsb in
+  let rsapmsId = PMS.RSAPMS(pk, pv, rsapms) in
+  let ns =
+    if ems then
+      C_12_wait_MS csr alpha rsapmsId pmsb
+    else
+      let kef = kefAlg pv cs false in
+      let ms = TLSPRF.extract kef pmsb csr 48 in
+      dbg ("master secret: "^print_bytes ms);
+      let msId = StandardMS rsapmsId csr kef in
+      C_12_has_MS csr alpha msId ms in
+  ns, encrypted
+
+// second call from client_ServerHelloDone
+val client12_set_session_hash: 
+  st: ks_client_state -> 
+  h:bytes -> ST (ks_client_state * TLSPRF.key * recordInstance)
+  (requires fun h0 ->
+    C_12_wait_MS? st \/ C_12_has_MS? st)
+  (ensures fun h0 (st,prfk,ak) h1 ->
+    C_12_has_MS? st /\ 
+    modifies_none h0 h1)
+
+let client12_set_session_hash st log =
+  dbg ("client12_set_session_hash hashed_log = "^print_bytes log);
+  let st, ms =
+    match st with
+    | C_12_has_MS csr alpha msId ms ->
+      dbg ("master secret:"^print_bytes ms);
+      st, ms
+    | C_12_wait_MS csr alpha pmsId pms ->
+      let (pv, cs, ems) = alpha in
+      let kef = kefAlg pv cs ems in
+      let h = verifyDataHashAlg_of_ciphersuite cs in
+      let msId, ms =
+        if ems then
+          begin
+          let ms = TLSPRF.prf (pv,cs) pms (utf8 "extended master secret") log 48 in
+          dbg ("extended master secret:"^print_bytes ms);
+          let msId = ExtendedMS pmsId log kef in
+          msId, ms
+          end
+        else
+          begin
+          let ms = TLSPRF.extract kef pms csr 48 in
+          dbg ("master secret:"^print_bytes ms);
+          let msId = StandardMS pmsId csr kef in
+          msId, ms
+          end
+      in
+      C_12_has_MS csr alpha msId ms, ms
+      ms
+    in
+  let appk = ks_12_record_key ks in
+  (st, TLSPRF.coerce ms, appk)
+
+// *********************************************************************************
+//  All functions below assume that the MS is already computed (and thus they are
+//  shared accross role, key exchange, handshake mode...)
+// *********************************************************************************
+
+(*)
+let client12_client_finished ks
+  : ST (cvd:bytes)
+  (requires fun h0 ->
+    let st = sel h0 (KS?.state ks) in
+    C? st /\ C_12_has_MS? (C?.s st))
+  (ensures fun h0 r h1 -> h1 == h0)
+  =
+  let KS #region st = ks in
+  let C (C_12_has_MS csr alpha msId ms) = !st in
+  let (pv, cs, ems) = alpha in
+//  let h = verifyDataHashAlg_of_ciphersuite cs in
+//  let log = HandshakeLog.getHash hsl h in
+  let log = HandshakeLog.getBytes hsl in
+  TLSPRF.verifyData (pv,cs) ms Client log
+
+let server12_client_finished ks
+  : ST (cvd:bytes)
+  (requires fun h0 ->
+    let st = sel h0 (KS?.state ks) in
+    S? st /\ S_12_has_MS? (S?.s st))
+  (ensures fun h0 r h1 -> h1 == h0)
+  =
+  let KS #region st = ks in
+  let S (S_12_has_MS csr alpha msId ms) = !st in
+  let (pv, cs, ems) = alpha in
+//  let h = verifyDataHashAlg_of_ciphersuite cs in
+//  let log = HandshakeLog.getHash hsl h in
+  let log = HandshakeLog.getBytes hsl in
+  TLSPRF.verifyData (pv,cs) ms Client log
+
+let server12_server_finished ks
+  : ST (svd:bytes)
+  (requires fun h0 ->
+    let st = sel h0 (KS?.state ks) in
+    S? st /\ S_12_has_MS? (S?.s st))
+  (ensures fun h0 r h1 ->
+    let KS #rid st = ks in
+    modifies (Set.singleton rid) h0 h1
+    /\ modifies_rref rid !{as_ref st} (HS.HS?.h h0) (HS.HS?.h h1))
+  =
+  let KS #region st = ks in
+  let S (S_12_has_MS csr alpha msId ms) = !st in
+  let (pv, cs, ems) = alpha in
+//  let h = verifyDataHashAlg_of_ciphersuite cs in
+//  let log = HandshakeLog.getHash hsl h in
+  let log = HandshakeLog.getBytes hsl in
+  st := S S_Done;
+  TLSPRF.verifyData (pv,cs) ms Server log
+
+let client12_server_finished ks
+  : ST (svd:bytes)
+  (requires fun h0 ->
+    let st = sel h0 (KS?.state ks) in
+    C? st /\ C_12_has_MS? (C?.s st))
+  (ensures fun h0 r h1 ->
+    let KS #rid st = ks in
+    modifies (Set.singleton rid) h0 h1
+    /\ modifies_rref rid !{as_ref st} (HS.HS?.h h0) (HS.HS?.h h1))
+  =
+  let KS #region st = ks in
+  let C (C_12_has_MS csr alpha msId ms) = !st in
+  let (pv, cs, ems) = alpha in
+//  let h = verifyDataHashAlg_of_ciphersuite cs in
+//  let log = HandshakeLog.getHash hsl h in
+  let log = HandshakeLog.getBytes hsl in
+  st := C C_Done;
+  TLSPRF.verifyData (pv,cs) ms Server log
+*)
+
+val getId: recordInstance -> GTot id
+let getId (StAEInstance #i rd wr) = i
+
+--- *)
