src/tls/IV.fst
@@ -1,0 +1,81 @@
+module IV
+
+//17-12-08 to be adjusted; not sure we need a flag for it.
+
+open Mem
+open Pkg 
+
+let sample (len:UInt32.t): ST (lbytes len)
+    (requires fun h0 -> True)
+    (ensures fun h0 r h1 -> h0 == h1)
+  = CoreCrypto.random (UInt32.v len)
+
+
+/// A sample functionality for fresh, public initialization vectors,
+/// with the length of the byte vector as a basic agility
+/// parameter. We use this functionality e.g. for generating the
+/// static IV for TLS AEAD as part of the TLS key schedule.
+/// 
+/// There is no proper idealization flags here; the main
+/// (unconditional) property is that the vector is a function of the
+/// index; this vector is fresh whenever create is called instead of
+/// coerce.
+
+// should be set together with its parent KDF.
+assume val flag_Raw: b:bool{b ==> model}
+type idealRaw = b2t flag_Raw
+
+type rawlen (#ip: ipkg) (#len_of_i: ip.t -> keylen) (i:ip.t) = len:keylen {len = len_of_i i}
+type raw (ip: ipkg) (len_of_i: ip.t -> keylen) (i:ip.t{ip.registered i}) = lbytes (len_of_i i)
+
+let shared_footprint_raw (ip: ipkg) (len_of_i: ip.t -> keylen): rset = Set.empty
+
+let footprint_raw (ip: ipkg) (len_of_i: ip.t -> keylen)
+  (#i:ip.t {ip.registered i}) (k:raw ip len_of_i i)
+  : GTot (s:rset{s `Set.disjoint` shared_footprint_raw ip len_of_i})
+  =
+  let fp = Set.empty in
+  assume(fp `Set.disjoint` shared_footprint_raw ip len_of_i);
+  fp
+
+let create_raw (ip: ipkg) (len_of_i: ip.t -> keylen)
+  (i:ip.t{ip.registered i}) (len:keylen {len = len_of_i i}):
+  ST (raw ip len_of_i i)
+  (requires fun h0 -> model)
+  (ensures fun h0 p h1 -> modifies_none h0 h1)
+  = sample len
+
+let coerceT_raw (ip: ipkg) (len_of_i: ip.t -> keylen)
+  (i: ip.t {ip.registered i /\ (idealRaw ==> ~(ip.honest i))})
+  (len:keylen {len = len_of_i i}) (r:lbytes len):
+  GTot (raw ip len_of_i i) = r
+
+let coerce_raw (ip: ipkg) (len_of_i: ip.t -> keylen)
+  (i: ip.t {ip.registered i /\ (idealRaw ==> ~(ip.honest i))})
+  (len:keylen {len = len_of_i i}) (r:lbytes len):
+  ST (raw ip len_of_i i)
+  (requires fun h0 -> True)
+  (ensures fun h0 k h1 -> k == coerceT_raw ip len_of_i i len r /\ modifies_none h0 h1)
+  = r
+
+let local_raw_pkg (ip:ipkg) (len_of_i: ip.t -> keylen) : local_pkg ip =
+  LocalPkg
+    (raw ip len_of_i)
+    (rawlen #ip #len_of_i)
+    (fun #i (n:rawlen i) -> n)
+    idealRaw
+    (shared_footprint_raw ip len_of_i)
+    (footprint_raw ip len_of_i)
+    (fun #_ _ _ -> True) // no invariant
+    (fun _ _ _ _ _ -> ())
+    (fun #_ _ _ _ -> True) // no post-condition
+    (fun #_ _ _ _ _ _ -> ())
+    (create_raw ip len_of_i)
+    (coerceT_raw ip len_of_i)
+    (coerce_raw ip len_of_i)
+
+let rp (ip:ipkg) (len_of_i: ip.t -> keylen): ST (pkg ip)
+  (requires fun h0 -> True)
+  (ensures fun h0 p h1 -> modifies_one tls_define_region h0 h1 /\ p.package_invariant h1)
+  =
+  memoization_ST (local_raw_pkg ip len_of_i)
