src/tls/Idx.fst
@@ -1,0 +1,228 @@
+module Idx
+
+open Mem
+open Pkg
+
+module MR = FStar.Monotonic.RRef
+module MM = FStar.Monotonic.Map
+
+// 17-12-08 we considered separating "honesty" from the more ad hoc parts of this file.
+
+/// TLS-SPECIFIC KEY INDICES
+/// --------------------------------------------------------------------------------------------------
+///
+/// We provide an instance of ipkg to track key derivation (here using constant labels)
+/// these labels are specific to HKDF, for now strings e.g. "e exp master".
+type label = string
+
+/// the middle extraction takes an optional DH secret, identified by this triple
+/// we use our own datatype to simplify typechecking
+type id_dhe =
+  | NoIDH
+  | IDH:
+    gX: CommonDH.dhi ->
+    gY: CommonDH.dhr gX -> id_dhe
+
+// The "ciphersuite hash algorithms" eligible for TLS 1.3 key derivation.
+// We will be more restrictive.
+type kdfa = Hashing.Spec.alg
+
+/// Runtime key-derivation parameters, to be adjusted.
+///
+/// HKDF defines an injective function from label * context to bytes, to be used as KDF indexes.
+///
+type context =
+  | Extract: context // TLS extractions have no label and no context; we may separate Extract0 and Extract2
+  | ExtractDH: v:id_dhe -> context // This is Extract1 (the middle extraction)
+  | Expand: context // TLS expansion with default hash value
+  | ExpandLog: // TLS expansion using hash of the handshake log
+    info: TLSInfo.logInfo (* ghost, abstract summary of the transcript *) ->
+    hv: Hashing.Spec.anyTag (* requires stratification *) -> context
+
+/// Underneath, HKDF takes a "context" and a required length, with
+/// disjoint internal encodings of the context:
+/// [HKDF.format #ha label digest len]
+
+type id_psk = nat // external application PSKs only; we may also set the usage's maximal recursive depth here.
+type pre_id =
+  | Preshared:
+      a: kdfa (* fixing the hash algorithm *) ->
+      id_psk  ->
+      pre_id
+  | Derive:
+      i:pre_id (* parent index *) ->
+      l:label (* static part of the derivation label *) ->
+      context (* dynamic part of the derivation label *) ->
+      pre_id
+
+// always bound by the index (and also passed concretely at creation-time).
+val ha_of_id: i:pre_id -> kdfa
+let rec ha_of_id = function
+  | Preshared a _ -> a
+  | Derive i lbl ctx -> ha_of_id i
+
+// placeholders
+assume val idh_of_log: TLSInfo.logInfo -> id_dhe
+assume val summary: bytes -> TLSInfo.logInfo
+
+// concrete transcript digest
+let digest_info (a:kdfa) (info:TLSInfo.logInfo) (hv: Hashing.Spec.anyTag) =
+  exists (transcript: bytes).
+    // Bytes.length hv = tagLen a /\
+    hv = Hashing.Spec.hash a transcript /\
+    Hashing.CRF.hashed a transcript /\
+    info = summary transcript
+
+/// stratified definition of id required.
+///
+/// we will enforce
+/// * consistency on the hash algorithm
+/// * monotonicity of the log infos (recursively including earlier resumption logs).
+/// * usage restriction: the log after DH must include the DH identifier of the parent.
+///   (Hence, we should either forbid successive DHs or authenticate them all.)
+///
+val wellformed_id: pre_id -> Type0
+let rec wellformed_id = function
+  | Preshared a _ -> True
+  | Derive i l (ExpandLog info hv) -> wellformed_id i /\ digest_info (ha_of_id i) info hv
+  | Derive i lbl ctx ->
+      //TODO "ctx either extends the parent's, or includes its idh" /\
+      wellformed_id i
+
+type id = i:pre_id {wellformed_id i}
+
+type honest_idh (c:context) =
+  ExtractDH? c /\ IDH? (ExtractDH?.v c) /\
+  (let ExtractDH (IDH gX gY) = c in CommonDH.honest_dhr gY)
+
+/// We use a global honesty table for all indexes Inside ipkg, we
+/// assume all index types are defined in the table below We assume
+/// write access to this table is public, but the following global
+/// invariant must be enforced: if i is corrupt then all indexes
+/// derived from i are also corrupt
+/// ---EXCEPT if ctx is ExtractDH g gx gy with CommonDH.honest_dhr gy
+///
+type honesty_invariant (m:MM.map' id (fun _ -> bool)) =
+  (forall (i:id) (l:label) (c:context{wellformed_id (Derive i l c)}).
+  {:pattern (m (Derive i l c))}
+  Some? (m (Derive i l c)) ==> Some? (m i) /\
+  (m i = Some false ==> (honest_idh c \/ m (Derive i l c) = Some false)))
+
+//17-12-08 removed [private] twice, as we need to recall it in ODH :(
+type i_honesty_table =
+  MM.t tls_honest_region id (fun (t:id) -> bool) honesty_invariant
+let h_table = if model then i_honesty_table else unit
+
+let honesty_table: h_table =
+  if model then
+    MM.alloc #tls_honest_region #id #(fun _ -> bool) #honesty_invariant
+  else ()
+
+// Registered is monotonic
+type registered (i:id) =
+  (if model then
+    let log : i_honesty_table = honesty_table in
+    MR.witnessed (MM.defined log i)
+  else True)
+
+type regid = i:id{registered i}
+
+type honest (i:id) =
+  (if model then
+    let log: i_honesty_table = honesty_table in
+    MR.witnessed (MM.contains log i true)
+  else False)
+
+type corrupt (i:id) =
+  (if model then
+    let log : i_honesty_table = honesty_table in
+    MR.witnessed (MM.contains log i false)
+  else True)
+
+// ADL: difficult to prove, relies on an axiom outside the current formalization of FStar.Monotonic
+let lemma_honest_corrupt (i:regid)
+  : Lemma (honest i <==> ~(corrupt i)) =
+  admit()
+
+let lemma_corrupt_invariant (i:regid) (lbl:label)
+  (ctx:context {wellformed_id (Derive i lbl ctx) /\ registered (Derive i lbl ctx)})
+  : ST unit
+  (requires fun h0 -> ~(honest_idh ctx))
+  (ensures fun h0 _ h1 ->
+    corrupt i ==> corrupt (Derive i lbl ctx) /\ h0 == h1)
+  =
+  lemma_honest_corrupt i;
+  lemma_honest_corrupt (Derive i lbl ctx);
+  if model then
+    let log : i_honesty_table = honesty_table in
+    MR.m_recall log;
+    MR.testify (MM.defined log i);
+    match MM.lookup log i with
+    | Some true -> ()
+    | Some false ->
+      let m = MR.m_read log in
+      // No annotation, but the proof relies on the global log invariant
+      MR.testify (MM.defined log (Derive i lbl ctx));
+      MM.contains_stable log (Derive i lbl ctx) false;
+      MR.witness log (MM.contains log (Derive i lbl ctx) false)
+  else ()
+
+let get_honesty (i:id {registered i}) : ST bool
+  (requires fun h0 -> True)
+  (ensures fun h0 b h1 -> h0 == h1 /\ (b <==> honest i))
+  =
+  lemma_honest_corrupt i;
+  if model then
+    let log : i_honesty_table = honesty_table in
+    MR.m_recall log;
+    MR.testify (MM.defined log i);
+    match MM.lookup log i with
+    | Some b -> b
+  else false
+
+// TODO(adl) preservation of the honesty table invariant
+let rec lemma_honesty_update (m:MM.map id (fun _ -> bool) honesty_invariant)
+  (i:regid) (l:label) (c:context{wellformed_id (Derive i l c)}) (b:bool{b <==> honest i})
+  : Lemma (honesty_invariant (MM.upd m (Derive i l c) b))
+// : Lemma (requires Some? (m i ) /\ None? (m (Derive i l c)) /\ m i == Some false ==> not b)
+//         (ensures honesty_invariant (MM.upd m (Derive i l c) b))
+  = admit() // easy
+
+let register_derive (i:id{registered i}) (l:label) (c:context{wellformed_id (Derive i l c)})
+  : ST (i:id{registered i} * bool)
+  (requires fun h0 -> True)
+  (ensures fun h0 (i', b) h1 ->
+    (if model then modifies_one tls_honest_region h0 h1 else h0 == h1)
+    /\ (i' == Derive i l c)
+    /\ (b2t b <==> honest i'))
+  =
+  let i':id = Derive i l c in
+  if model then
+    let log : i_honesty_table = honesty_table in
+    MR.m_recall log;
+    match MM.lookup log i' with
+    | Some b -> lemma_honest_corrupt i'; (i', b)
+    | None ->
+      let b = get_honesty i in
+      let h = get () in
+      lemma_honesty_update (MR.m_sel h log) i l c b;
+      MM.extend log i' b;
+      lemma_honest_corrupt i';
+      (i', b)
+  else (i', false)
+
+// 17-10-21 WIDE/NARROW INDEXES (old)
+//
+// We'd rather keep wide indexes secret.  Internally, for each salt
+// index, we maintain a table from (g, gX, gY) to PRFs, with some
+// sharing.  (The sharing may be public, but not wide indexes values
+// are not.)  Informally this is sound because our limited use of the
+// tables does not depend on their sharing.
+//
+// The danger of overly precise indexes is that, ideally, we may
+// separate instances that use the same concrete keys---in our case
+// this does not matter because security does not depend on their
+// sharing.
+
+let ii: ipkg = // (#info:Type0) (get_info: id -> info) =
+  Idx id registered honest get_honesty
