src/tls/KDF.Rekey.fst
@@ -1,0 +1,163 @@
+module KDF.Rekey
+
+open Mem
+open Pkg
+open Idx 
+open Pkg.Tree
+
+include AEAD.Pkg
+include KDF 
+
+/// This file illustrates our use of indexes, packages, and KDF on a
+/// simple recursive subset of the TLS key-schedule: late rekeying. It
+/// also provides a standalone test for verification and extraction.
+
+//17-11-15 for testing; rename to aeadAlg_of_id ?
+assume val get_aeadAlg: i:id -> aeadAlg
+let derive_aea
+  (lbl:label) (i:id)
+  (a:info{wellformed_id (Derive i lbl Expand)}):
+  (a':aeadAlg{a' == get_aeadAlg (Derive i lbl Expand)})
+=
+  //fixme! should be extracted from a
+  get_aeadAlg (Derive i lbl Expand)
+
+let is_ae_p (p: pkg ii) =
+  Pkg?.key p == key ii get_aeadAlg /\ p == memoization (local_ae_pkg ii get_aeadAlg) p.define_table
+let is_kdf_p (p: pkg ii) d children = // same as ksd_subtree
+  Pkg?.key p == secret d children /\ p == memoization (local_kdf_pkg d children) p.define_table
+
+// this function should specify enough to call key derivations.
+let rec is_secret (n:nat) (x:tree (idealKDF n)) =
+  if n = 0 then
+    match x with
+    | Node p [] -> is_kdf_p p 0 []
+    | _ -> False
+  else
+    match x with
+    | Node p ["AE",Leaf ae; "RE",re ] ->
+      lemma_KDF_depth n;
+      is_kdf_p p n ["AE",Leaf ae; "RE", re] /\
+      is_ae_p ae /\ is_secret (n-1) re
+    | _ -> False
+
+// let is_secret_shape (n:nat) (x:tree {is_secret n x}): Lemma (Node? x) =
+//   if n = 0 then () else ()
+
+
+assume val mk_kdf: d:nat -> u:usage d -> ST (pkg ii)
+  (requires fun h0 -> True)
+  (ensures fun h0 p h1 -> is_kdf_p p d u)
+
+// this function allocates all tables and (WIP) sets up the initial invariant.
+val mk_secret (n:nat): ST (tree (idealKDF n))
+  (requires fun h0 -> True)
+  (ensures fun h0 x h1 ->
+    is_secret n x /\
+    True // tree_invariant x h1 // requires finer posts for mp pp etc
+    )
+
+let rec mk_secret n =
+  if n = 0 then (
+    assume(valid_children (idealKDF 0) []);
+    let c : usage 0 = [] in
+    let p = mk_kdf 0 c in
+    Node p c
+  ) else (
+    let ae = mp ii get_aeadAlg in
+    assume(is_ae_p ae);// should be in the post of mp.
+    lemma_KDF_depth n;
+    let re = mk_secret (n-1) in
+    assert(is_secret (n-1) re);
+    let children = [ "AE",Leaf ae; "RE",re ] in
+    assume(valid_children (idealKDF n) children);
+    let p = mk_kdf n children in
+    assert(is_kdf_p p n [ "AE",Leaf ae; "RE",re ]);
+    Node p children)
+
+//#set-options "--z3rlimit 200"
+#set-options "--lax"
+let test_rekey(): St unit
+=
+  let x0 = mk_secret 10 in
+  let h0 = get() in
+  assert(is_secret 10 x0);
+  assume(tree_invariant x0 h0); // soon a post of mk_secret
+
+  match x0 with
+  | Node pkg0 ["AE",Leaf aepkg1; "RE",x1 ] -> (
+    let children0 : usage 10 = ["AE",Leaf aepkg1; "RE",x1 ] in
+    assert(u_of_t (x0 <: kdf_subtree 10) == children0);
+
+    let a0 = Info Hashing.Spec.SHA1 None in
+    let i0: i:id {registered i /\ a0 = get_info i} = magic() in
+    assert(is_kdf_p pkg0 10 children0);
+
+    assert(pkg0.package_invariant h0 /\ tree_invariant x1 h0);
+    // create's pre; should follow from pkg0's package invariant
+    assume(model /\ mem_fresh pkg0.define_table i0 h0);
+    assert(Pkg?.key pkg0 == secret 10 children0);
+
+    let s0: secret 10 children0 i0 = (Pkg?.create pkg0) i0 a0 in
+
+    assert(is_secret 9 x1);
+
+    match x1 with
+    | Node pkg1 ["AE",Leaf aepkg2; "RE",x2] -> (
+      let children1 : usage 9 = ["AE",Leaf aepkg2; "RE",x2 ] in
+      let a1 = Info Hashing.Spec.SHA1 None in
+      let h1 = get() in
+
+      assume(tree_invariant x0 h0 ==> tree_invariant x0 h1); // tree_invariant_frame
+
+      let (|_,s1|) = derive #10 #(x0 <: kdf_subtree 10) s0 a0 "RE" Expand a1 in
+      let i1: regid = Derive i0 "RE" Expand in
+
+      let s1: secret 9 children1 i1 = s1 in
+      let aea = derive_aea "AE" i1 a1 in
+      let h2 = get() in
+
+      assume(tree_invariant x1 h2);
+
+      let (|_,k1|) = derive #9 #(x1 <: kdf_subtree 9) s1 a1 "AE" Expand aea in
+      let ik1: regid = Derive i1 "AE" Expand in
+      let k1: key ii get_aeadAlg ik1 = k1 in
+      let h3 = get() in
+      assume(aead_inv k1 h3); // should follow from the multi-pkg invariant
+
+      let cipher = encrypt ii get_aeadAlg #ik1 k1 42 in
+
+      // assert(tree_invariant x1);
+      // assert(tree_invariant x0);
+      () ))
+//    | _ -> assert false) // excluded by is_secret 9
+//  |  _ -> assert false // excluded by is_secret 10
+// refactoring needed, e.g. define derive_secret helper function to hide access to the tree
+
+(*
+let modifies_instance
+  (i: id {wellformed_id i})
+  (p: localpkg ii)
+  (k: key i)
+  (h0 h1: mem)
+  (modifies_local: modifies (p.local_footprint k) h0 h1)
+  (inv0: inv_node u h0):
+  Lemma (inv_node u h1) =
+
+let rec step u j i =
+
+// from the post of a key derivation, we should have our framing lemma.
+
+let rec descend u j i = // j decreases
+  j = i \/
+  match j with
+  | Derive j0 lbl ctx -> derived j0 i
+  | Preshared -> False
+
+  match j, i with
+  | Preshared
+
+  i = j \/
+  exists (lbl, ctx). derived (Derive i lbl ctx)
+*)
+
