src/tls/KDF.fst
@@ -1,0 +1,529 @@
+module KDF
+
+/// We define a KDF parametric in both its usage and ipkg
+/// We rely on type abstraction to separate secrets with different indexes
+/// For soundness, we must also prevent external calls to create derived secrets.
+///
+/// We idealize KDF as a random function, with lazy sampling.
+/// This holds syntactically only after inlining all calls to
+/// pkg.create/coerce.
+///
+/// This requires memoizing calls, which is a bit tricky when calling
+/// stateful allocators.
+
+open Mem
+open Pkg
+open Idx 
+open Pkg.Tree
+
+module MR = FStar.Monotonic.RRef
+module MM = FStar.Monotonic.Map
+module HH = FStar.HyperHeap
+module HS = FStar.HyperStack
+
+let sample (len:UInt32.t): ST (lbytes len)
+    (requires fun h0 -> True)
+    (ensures fun h0 r h1 -> h0 == h1)
+  = CoreCrypto.random (UInt32.v len)
+
+
+
+assume val flag_KDF: d:nat -> b:bool{b ==> model}
+type idealKDF d = b2t (flag_KDF d)
+assume val lemma_KDF_depth: d:nat{d>0} -> Lemma (idealKDF d ==> idealKDF (d-1))
+
+// Note that when model is off, safeKDF is False
+type safeKDF (d:nat) (i:id{registered i}) = idealKDF d /\ honest i
+
+// KDF-specific usage: the parent property is idealKDF at level d
+type usage (d:nat) = children (idealKDF d)
+
+type details (ha:kdfa) = | Log:
+  loginfo: TLSInfo.logInfo ->
+  hv: Hashing.Spec.anyTag {digest_info ha loginfo hv} -> details ha
+
+type info = | Info:
+  ha:kdfa ->
+  option (details ha) -> info
+
+val get_info: id -> info
+// 17-11-01 can't get it to verify; should follow from the definition of wellformed_id?
+//#set-options "--initial_ifuel 2 --initial_fuel 2"
+let rec get_info (i0: id): info =
+  match i0 with
+  | Preshared a _                 -> Info a None
+  | Derive i l (ExpandLog log hv) -> Info (ha_of_id i) (Some (Log log hv))
+  | Derive i _ _                  -> get_info i
+
+assume val hkdf_derive_label_spec:
+  ha: Hashing.Spec.alg -> k: Hashing.Spec.tag ha -> lbl: label -> ctx:context -> GTot (Hashing.Spec.tag ha)
+
+let derived_key
+  (d: nat)
+  (u: usage d)
+  (i: regid)
+  (lbl: label {u `has_lbl` lbl})
+  (ctx: context {wellformed_id (Derive i lbl ctx) /\ registered (Derive i lbl ctx)})
+  =
+  (Pkg?.key (child u lbl)) (Derive i lbl ctx)
+
+let kdf_tables_region : tls_rgn = new_region Mem.tls_tables_region
+
+/// key-derivation table (memoizing create/coerce)
+type domain (d:nat) (u:usage d) (i:id{registered i}) = | Domain:
+  lbl: label {u `has_lbl` lbl} ->
+  ctx: context {wellformed_id (Derive i lbl ctx) /\ registered (Derive i lbl ctx)} ->
+  domain d u i
+
+type kdf_range (de:nat) (u:usage de) (i:id{registered i}) (d:domain de u i) =
+  (let Domain lbl ctx = d in derived_key de u i lbl ctx)
+
+type ideal_or_real (it:Type0) (rt:Type0) =
+  | Ideal: v:it -> ideal_or_real it rt
+  | Real: v:rt -> ideal_or_real it rt
+
+unfold type ir_key (safe: i:id{registered i} -> GTot Type0) (it:Type0) (rt:Type0) (i:regid) =
+  (if model then
+    s:ideal_or_real it rt{safe i <==> Ideal? s}
+  else rt)
+
+noeq private type table (d:nat) (u:usage d) (i:id{registered i}) =
+  | KDF_table:
+    r:subrgn kdf_tables_region ->
+    t:MM.t r (domain d u i) (kdf_range d u i) (fun _ -> True) ->
+    table d u i
+
+let secret_len (a:info) : keylen = UInt32.uint_to_t (Hashing.Spec.tagLen a.ha)
+type real_secret (i:id{registered i}) = lbytes (secret_len (get_info i))
+
+// id vs regid?
+type secret (d:nat) (u:usage d) (i:id{registered i}) =
+  ir_key (safeKDF d) (table d u i) (real_secret i) i
+
+// when to be parametric on ip? not for the KDF itself: we use ip's constructors.
+//type secret (u: usage info) (i:regid) =
+//  (if honest i then table u i
+//  else lbytes (secret_len (get_info i)))
+
+let secret_ideal (#d:nat) (#u: usage d) (#i:id{registered i}) (t: secret d u i {safeKDF d i}): table d u i =
+  let t : s:ideal_or_real (table d u i) (real_secret i) {safeKDF d i <==> Ideal? s} = t in
+  Ideal?.v t
+
+let ideal_secret (#d:nat) (#u: usage d) (#i:id{registered i}) (t: table d u i {safeKDF d i}) : secret d u i =
+  let t : s:ideal_or_real (table d u i) (real_secret i) {safeKDF d i <==> Ideal? s} = Ideal t in
+  assert(model); t
+
+let secret_corrupt (#d:nat) (#u: usage d) (#i:id{registered i}) (t: secret d u i {~(safeKDF d i)}): real_secret i =
+  if model then
+   let t : s:ideal_or_real (table d u i) (real_secret i) {safeKDF d i <==> Ideal? s} = t in
+   Real?.v t
+  else t
+
+let corrupt_secret (#d:nat) (#u: usage d) (#i:id{registered i}) (t: real_secret i {~(safeKDF d i)}) : secret d u i =
+  if model then
+    let s : s:ideal_or_real (table d u i) (real_secret i) {safeKDF d i <==> Ideal? s} = Real t in s
+  else t
+
+/// Real KDF schemes, parameterized by an algorithm computed from the
+/// index (existing code).
+
+let lemma_honest_parent (i:id{registered i}) (lbl:label)
+  (ctx:context {wellformed_id (Derive i lbl ctx) /\ registered (Derive i lbl ctx)})
+  : Lemma (requires ~(honest_idh ctx)) (ensures honest (Derive i lbl ctx) ==> honest i)
+  = admit() // hard, uses the monotonic excluded middle axiom and table invariant
+
+// For KDF, we require that being fresh in the KDF table implies being fresh
+// in the derived package's definition table
+type local_kdf_invariant (#d:nat) (#u:usage d) (#i:id{registered i}) (k:secret d u i) (h:mem) =
+  (forall (lbl:label {u `has_lbl` lbl}) (ctx':context).
+    (~(honest_idh ctx') /\ wellformed_id (Derive i lbl ctx') /\ registered (Derive i lbl ctx')) ==>
+      (let ctx : c:context{wellformed_id (Derive i lbl c) /\ registered (Derive i lbl c)} = ctx' in
+      let i' : i:id{registered i} = Derive i lbl ctx in
+      lemma_honest_parent i lbl ctx;
+      let pkg' = child u lbl in
+      // Nice: we get this from the tree structure for free!
+      assert(Pkg?.ideal pkg' ==> idealKDF d);
+      (if model then
+        let dt = itable pkg'.define_table in
+        let kdf : ir:ideal_or_real (table d u i) (real_secret i) {safeKDF d i <==> Ideal? ir} = k in
+        // We need this for coerce
+        assert(safeKDF d i <==> Ideal? kdf);
+        match kdf with
+        | Ideal kdft ->
+          // the entries in the KDF table match those of the child's define_table
+          let KDF_table r t : table d u i = kdft in
+          MM.sel (MR.m_sel h t) (Domain lbl ctx) == MM.sel (MR.m_sel h dt) i'
+        | Real raw ->
+          assert(~(safeKDF d i));
+          assert(honest i' ==> honest i);
+          assert(Pkg?.ideal pkg' ==> ~(honest i')); // to call coerceT
+          // the child's define table has correctly-computed coerced entries
+          (match MM.sel (MR.m_sel h dt) i' with
+          | None -> True
+          | Some k' ->
+            // we recompute the concrete key materials, and recall the
+            // existence of some prior info, which (by specification
+            // of coerceT) must yield exactly the same instance as the
+            // one recorded earlier.
+            let i'': i:id{registered i /\ (Pkg?.ideal pkg' ==> ~(honest i))} = i' in
+            let raw' = hkdf_derive_label_spec (get_info i).ha raw lbl ctx in
+            exists (a':Pkg?.info pkg' i').
+            Pkg?.len pkg' a' == UInt32.uint_to_t (Hashing.Spec.tagLen (get_info i).ha) /\
+            k' == Pkg?.coerceT pkg' i'' a' raw')
+      else True)))
+
+let kdf_shared_footprint (#d:nat) (u:usage d) : rset =
+  assume false; Set.empty
+  // List.Tot.fold_left (Set.empty) (fun s p -> rset_union s p.define_region) u
+
+let kdf_footprint (#d:nat) (#u:usage d) (#i:id{registered i}) (k:secret d u i)
+  : GTot (s:rset{s `Set.disjoint` kdf_shared_footprint u}) =
+  assume false; // WIP(adl) Fix rset for define_region subrgn
+  if model then
+    let k : ideal_or_real (table d u i) (real_secret i) = k in
+    match k with
+    | Ideal (KDF_table r _) -> Set.singleton r
+    | Real k -> Set.empty
+  else Set.empty
+
+let local_kdf_invariant_framing (#d:nat) (#u:usage d) (i:id{registered i}) (k:secret d u i) (h0:mem) (r:HH.rid) (h1:mem)
+  : Lemma (requires local_kdf_invariant k h0 /\ modifies_one r h0 h1
+            /\ ~(r `Set.mem` kdf_footprint k) /\ ~(r `Set.mem` kdf_shared_footprint u))
+          (ensures local_kdf_invariant k h1)
+  = admit()
+
+/// maybe reverse-inline sampling from low-level KeyGen?
+/// otherwise we have to argue it is what Create does.
+///
+/// MK: what does reverse-inline of low-level KeyGen mean?
+
+// The post-condition of creating a KDF is that its table is empty
+// This is useful to re-establish the multi-KDF invariant
+type kdf_post (#d:nat) (#u:usage d) (#i:id{registered i}) (a: info {a == get_info i}) (k:secret d u i) (h:mem) =
+  (safeKDF d i ==>
+    (let KDF_table r t = secret_ideal k in
+     MR.m_sel h t == MM.empty_map (domain d u i) (kdf_range d u i)))
+
+// Framing for the kdf_post depends only on kdf_footprint k
+let kdf_post_framing (#d:nat) (#u:usage d) (#i:id{registered i}) (a: info {a == get_info i})
+  (k:secret d u i) (h0:mem) (r:HH.rid) (h1:mem)
+  : Lemma (requires (kdf_post a k h0 /\ modifies_one r h0 h1 /\ ~(r `Set.mem` kdf_footprint k)))
+          (ensures (kdf_post a k h1))
+  = admit()
+
+val coerceT:
+  d: nat ->
+  u: usage d ->
+  i: id{registered i /\ ~(safeKDF d i)} ->
+  a: info {a == get_info i} (* run-time *) ->
+  repr: lbytes (secret_len a) ->
+  GTot (secret d u i)
+let coerceT d u i a repr =
+  corrupt_secret #d #u #i repr
+
+val coerce:
+  d: nat ->
+  u: usage d ->
+  i: id{registered i /\ ~(safeKDF d i)} ->
+  a: info {a == get_info i} (* run-time *) ->
+  repr: lbytes (secret_len a) ->
+  ST (secret d u i)
+  (requires fun h0 -> True)
+  (ensures fun h0 k h1 -> modifies_none h0 h1
+    /\ k == coerceT d u i a repr
+    /\ fresh_regions (kdf_footprint k) h0 h1
+    /\ kdf_post a k h1 /\ local_kdf_invariant k h1)
+
+let coerce d u i a repr =
+  let k = corrupt_secret #d #u #i repr in
+  let h1 = get() in
+  // WIP stronger packaging
+  (if model then assume(local_kdf_invariant k h1));
+  k
+
+/// NS:
+/// MM.alloc is a stateful function with all implicit arguments
+/// F* will refuse to instantiate all those arguments, since implicit
+/// instantiation in F* should never result in an effect.
+///
+/// Stateful functions always take at least 1 concrete argument.
+///
+/// I added a unit here
+///
+/// CF: Ok; I did not know. Is it a style bug in FStar.Monotonic.Map ?
+let alloc #a #b #inv (r:FStar.Monotonic.RRef.rid)
+  : ST (MM.t r a b inv)
+       (requires (fun h -> inv (MM.empty_map a b)))
+       (ensures (fun h0 x h1 ->
+    inv (MM.empty_map a b) /\
+    ralloc_post r (MM.empty_map a b) h0 (FStar.Monotonic.RRef.as_hsref x) h1))
+  = MM.alloc #r #a #b #inv
+
+val create:
+  d: nat ->
+  u: usage d ->
+  i: id{registered i} -> // using regid yields unification failures below
+  a: info {a == get_info i}(* run-time *) ->
+  ST (secret d u i)
+  (requires fun h0 -> model)
+  (ensures fun h0 k h1 -> modifies_none h0 h1
+    /\ fresh_regions (kdf_footprint k) h0 h1
+    /\ kdf_post a k h1 /\ local_kdf_invariant k h1)
+
+let create d u i a =
+  let h0 = get() in
+  let honest = get_honesty i in
+  let h1 = get() in
+  if flag_KDF d && honest then
+   begin
+    assert(safeKDF d i);
+    let r : subrgn kdf_tables_region = new_region kdf_tables_region in
+    let h2 = get() in
+    assert(stronger_fresh_region r h1 h2);
+    let t : table d u i = KDF_table r (alloc r) in
+    let h3 = get() in
+    let k : secret d u i = ideal_secret t in
+    assume(kdf_footprint k == Set.singleton r);
+    assume(local_kdf_invariant k h3);
+    assert(fresh_regions (kdf_footprint k) h0 h3);
+    k
+   end
+  else
+   begin
+    let k = corrupt_secret #d #u #i (sample (secret_len a)) in
+    assume(local_kdf_invariant k h1); // TODO
+    k
+   end
+
+/// We are using many KDF packages (one for each usage),
+/// idealized one at a time.  (Having one proof step for each nested
+/// level of key derivation seems unavoidable: we need to idealize
+/// parents before childrens.)
+
+let local_kdf_pkg (d:nat) (u:usage d) : local_pkg ii =
+  (LocalPkg
+    (secret d u)
+    (fun i -> a:info{a == get_info i})
+    (fun #_ a -> secret_len a)
+    (idealKDF d)
+    (kdf_shared_footprint u)
+    (kdf_footprint #d #u)
+    (local_kdf_invariant #d #u)
+    (local_kdf_invariant_framing #d #u)
+    (kdf_post #d #u)
+    (kdf_post_framing #d #u)
+    (create d u)
+    (coerceT d u)
+    (coerce d u))
+
+let pp (d:nat) (u:usage d) : ST (pkg ii)
+  (requires fun h0 -> True)
+  (ensures fun h0 p h1 ->
+     modifies_mem_table p.define_table h0 h1 /\
+     p.package_invariant h1)
+  =
+  memoization_ST #ii (local_kdf_pkg d u)
+
+let ukey (d:nat) (u:usage d) (lbl:label {u `has_lbl` lbl}) (i:id{registered i}) =
+  Pkg?.key (child u lbl) i
+
+// Derive modifies:
+//  - the honesty table
+//  - the define table of the derived package
+//  - the KDF table
+// FIXME: can't use the normalizer to compute the set... destroys the implicit
+type modifies_derive (#d:nat) (#u:usage d) (#i:id{registered i}) (k:secret d u i)
+  (lbl:label {u `has_lbl` lbl}) (ctx:context {wellformed_id (Derive i lbl ctx)}) (h0:mem) (h1:mem) =
+  (if model then
+    let modset = Set.singleton tls_define_region in
+    let modset = Set.union modset (Set.singleton tls_honest_region) in
+    let k : ideal_or_real (table d u i) (real_secret i) = k in
+    let modset = match k with
+    | Ideal (KDF_table r _) -> Set.union modset (Set.singleton r)
+    | Real k -> modset in
+    let utable = (child u lbl).define_table in
+    modifies modset h0 h1
+    /\ HS.modifies_ref tls_define_region (Set.singleton (mem_addr (itable utable))) h0 h1
+  else modifies_none h0 h1) // FIXME concrete state
+
+
+//OLD
+let all_pkg_invariant h = forall (p:pkg ii). p.package_invariant h
+
+/// 17-11-30 experiment, testing package trees on a simple case: AEAD
+/// keying and forward re-keying; still unclear how to traverse the
+/// packaging.
+
+
+/// Global, generic invariant, to be rooted at the PSK
+/// (do we need some "static index"?)
+
+// node footprints already recursively collect their children's footprints
+let tree_footprint (x:tree') h : GTot rset =
+  match x with
+  | Leaf p -> Pkg?.footprint p h
+  | Node p c -> Pkg?.footprint p h
+// WIP: footprint_kdf includes the define tables of children, but not the package footprints
+//    rset_union (Pkg?.footprint p h)
+//      (List.Tot.fold_left (fun s p -> rset_union s (Pkg?.footprint p h)) c Set.empty)
+
+// library??
+val list_forall: ('a -> Type0) -> list 'a -> Tot Type0
+let rec list_forall f l = match l with
+    | [] -> True
+    | hd::tl -> f hd /\ list_forall f tl
+
+val disjoint_children: mem -> children' -> Type0
+let rec disjoint_children h = function
+  | [] -> True
+  | (l0, x0) :: tail -> list_forall (fun (l1, x1) -> tree_footprint x0 h `Set.disjoint` tree_footprint x1 h) tail
+
+(*
+/// SZ: An alternative way of defining [tree_invariant] without an ad-hoc termination measure
+
+val move_refinement: #a:Type -> #p:(a -> Type)
+  -> l:list a{forall z. List.Tot.memP z l ==> p z} -> list (x:a{p x})
+let rec move_refinement #a #p = function
+  | [] -> []
+  | hd :: tl -> hd :: move_refinement #a #p tl
+
+val forall_memP_precedes: #a:Type -> l:list a -> Lemma (forall x. List.Tot.memP x l ==> x << l)
+let forall_memP_precedes #a l =
+  let open FStar.Tactics in
+  let open FStar.List.Tot in
+  assert_by_tactic (forall x. memP x l ==> x << l)
+    (x <-- forall_intro; apply_lemma (quote memP_precedes))
+
+val precedes_list: #a:Type -> l:list a -> list (x:a{x << l})
+let precedes_list #a l = forall_memP_precedes l; move_refinement l
+
+val tree_invariant: mem -> tree -> Type0
+let rec tree_invariant h = function
+  | Leaf p -> Pkg?.package_invariant p h
+  | Node lxs p ->
+    Pkg?.package_invariant p h /\
+    list_forall (fun (p:(label * tree){p << lxs}) -> tree_invariant h (snd p)) (precedes_list lxs) /\
+    disjoint_children h lxs
+*)
+
+// another custom induction to get termination
+let rec children_forall
+  (lxs: children')
+  (f: x:tree'{depth x <= children_depth lxs} -> Type0): Type0
+=
+  match lxs with
+  | [] -> True
+  | (_,x)::tl ->
+    // children_depth tl <= children_depth lxs /\
+    // depth x <= children_depth lxs /\
+    f x /\ children_forall tl f
+
+let rec tree_invariant (x:tree') (h:mem): Tot Type0 (decreases %[depth x]) =
+  match x with
+  | Leaf p -> Pkg?.package_invariant p h
+  | Node p lxs ->
+    Pkg?.package_invariant p h /\
+    children_forall lxs (fun x -> tree_invariant x h) /\
+    disjoint_children h lxs
+
+// We can frame the multi-pkg invariant for free when touching tls_honest_region
+let tree_invariant_frame (t:tree') (h0:mem) (h1:mem)
+  : Lemma (requires tree_invariant t h0 /\ (modifies_none h0 h1 \/ modifies_one tls_honest_region h0 h1))
+          (ensures tree_invariant t h1)
+  = admit()
+
+// If we touch one package's footprint, but restore this package's invariant,
+// the multi-package invariant is restored
+let restore_all_pkg_invariant h0 (p:pkg ii) h1
+  : Lemma (requires all_pkg_invariant h0 /\ modifies (p.footprint h0) h0 h1 /\ p.package_invariant h1)
+          (ensures all_pkg_invariant h1)
+  = admit()
+
+// TODO 17-12-01 we need an hypothesis that captures that p is in the tree, e.g. only deal with the case where p is a child.
+
+type kdf_subtree (d:nat) = t:tree (idealKDF d){
+  Node? t /\ (let Node p u = t in
+  Pkg?.ideal p == idealKDF d /\
+  Pkg?.key p == LocalPkg?.key (local_kdf_pkg d u) /\
+  p == memoization (local_kdf_pkg d u) p.define_table)}
+
+let u_of_t (#d:nat) (t:kdf_subtree d) : usage d = Node?.children t
+let kdf_dt (#d:nat) (t:kdf_subtree d) : mem_table (secret d (u_of_t t)) = Pkg?.define_table (Node?.node t)
+
+/// The well-formedness condition on the derived label (opaque from
+/// the viewpoint of the KDF) enforces
+///
+inline_for_extraction
+val derive:
+  #d: nat ->
+  #t: kdf_subtree d ->
+  #i: id{registered i} ->
+  k: secret d (u_of_t t) i ->
+  a: info {a == get_info i} ->
+  lbl: label {(u_of_t t) `has_lbl` lbl} ->
+  ctx: context {~(honest_idh ctx) /\ wellformed_id (Derive i lbl ctx)} ->
+  a': Pkg?.info (child (u_of_t t) lbl) (Derive i lbl ctx) ->
+  ST (_:unit{registered (Derive i lbl ctx)} & ukey d (u_of_t t) lbl (Derive i lbl ctx))
+  // the second pre-condition is redundant, but we don't know the package of k
+  (requires fun h0 ->
+    mem_defined (kdf_dt t) i /\ // Need a witness that k is defined to get local_kdf_invariant
+    tree_invariant t h0)
+  (ensures fun h0 r h1 ->
+    modifies_derive k lbl ctx h0 h1 /\
+    tree_invariant t h1 /\
+    (Pkg?.post (child (u_of_t t) lbl)) a' (dsnd r) h1)
+
+let derive #d #t #i k a lbl ctx a' =
+  let u = u_of_t t in
+  let dt = kdf_dt t in
+
+  let h0 = get() in
+  let honest = get_honesty i in
+  let i', honest' = register_derive i lbl ctx in  // register (Derive i lbl ctx) and return its honesty
+  let h1 = get() in
+  // Frame the registration, only if model is one (otherwise h0 == h1)
+  tree_invariant_frame t h0 h1;
+
+  assume false; // WIP Dec 7
+
+  // Deduce from tree_invariant that local_kdf_invariant k h1 holds
+  if model then
+   begin
+    let log = itable dt in
+    MR.m_recall log;
+    let m = MR.m_sel h1 log in
+    assume(m i == Some k); // testify
+    lemma_mm_forall_elim m local_kdf_invariant i k h1;
+    assert(local_kdf_invariant k h1)
+   end;
+
+  lemma_corrupt_invariant i lbl ctx;
+  let x: domain d u i = Domain lbl ctx in
+  let pkg = child u lbl in
+  assert(Pkg?.ideal pkg ==> idealKDF d); // Nice!
+
+  if flag_KDF d && honest then
+   begin
+    let KDF_table kdf_r kdf_t : table d u i = secret_ideal k in
+    let v: option (derived_key d u i lbl ctx) = MM.lookup kdf_t x in
+    match v with
+    //17-10-30 was failing with scrutiny error: match MM.lookup (secret_ideal k) x
+    | Some dk -> (| (), dk |)
+    | None ->
+      let dk = Pkg?.create pkg i' a' in
+      let h2 = get() in
+      assume(tree_invariant t h2);
+      assert(mem_fresh pkg.define_table i' h2); // from kdf_local_inv
+      MM.extend kdf_t x dk;
+      (| (), dk |)
+   end
+  else
+   begin
+    let raw = HKDF.expand #(a.ha) (secret_corrupt k) (Platform.Bytes.abytes lbl) (UInt32.v (Pkg?.len pkg a')) in
+    let h2 = get() in
+    assume(modifies_none h1 h2); // FIXME HKDF framing
+    assume(tree_invariant t h2);
+    assert(Pkg?.ideal pkg ==> corrupt i');
+    let dk = Pkg?.coerce pkg i' a' raw in
+    (| (), dk |)
+   end
