src/tls/Pkg.fst
@@ -1,0 +1,437 @@
+module Pkg
+
+/// We develop a generic model for key extraction and key derivation
+/// parametrized by a usage function from labels to derived keyed
+/// functionalities.
+///
+/// * captures resumption derivations via bounded-recursive instantiation.
+/// * captures PRF-ODH double game
+/// * applicable to the full extract/expand key schedule of TLS 1.3
+/// * models partial key compromise, controlled by the adversary for each new key
+/// * features agility on hash algorithms and DH groups, and ideal-only indexes.
+///
+/// We first embed first-class modules as datatype "packages". This
+/// module specifies three kinds of packages (for indexes, local
+/// functionalities, and multi-instance functionalities) and provides
+/// generic "packaging" code from local packages to multi-instance
+/// packages.
+
+open Mem
+
+module MR = FStar.Monotonic.RRef
+module MM = FStar.Monotonic.Map
+module MH = FStar.Monotonic.Heap
+module HH = FStar.HyperHeap
+module HS = FStar.HyperStack
+
+let model = Flags.model
+
+type bytes = Platform.Bytes.bytes
+let lbytes (len:UInt32.t) = Platform.Bytes.lbytes (UInt32.v len)
+
+
+
+/// Index packages provide an abstract index for instances, with an
+/// interface to project (ghost) indexes to (concrete) runtime
+/// parameters, such as algorithms or key length , and to define their
+/// "honesty", thereby controlling their conditional idealization.
+///
+/// We distinguish between "honest", which refers to the adversary's
+/// intent (and is considered public) and "safe", which controls
+/// fine-grained idealization: roughly safe i = Flags.ideal /\ honest i
+
+noeq type ipkg = | Idx:
+  t: eqtype  (* abstract type for indexes *) ->
+  // three abstract predicates implemented as witnesses, and a stateful reader.
+  registered: (i:t -> GTot Type0) ->
+  honest: (i:t -> GTot Type0) ->
+  (* stateful reader, returning either honest or corrupt *)
+  get_honesty: (i:t{registered i} -> ST bool
+    (requires fun _ -> True)
+    (ensures fun h0 b h1 -> h0 == h1 /\ (b <==> honest i))) ->
+  ipkg
+
+
+/// Keyed functionality define Key packages, parametric in their
+/// indexes, but concrete on their key randomness. The package is
+/// meant to be used merely as a generic interface for
+/// creation/coercion; instances may have any number of other
+/// functions (such as leak, for instance).
+///
+/// [ip] defines the abstract indexes used in the package.
+///
+/// [info] represents creation-time information, such as algorithms or
+/// key lengths; it is largely determined by the (ghost) index, so
+/// that all users of the instance agree on them, with details left to
+/// each package definition. (For instance, parent regions for
+/// allocating ideal state may differ.) We pass both the index and its
+/// info inasmuch as the index will be erased.
+///
+/// [len] provides the concrete length of random key materials for
+/// creating a new instance, as a function of the creation-time info.
+///
+/// [create] and [coerce] generate new instances; [create] requires
+/// `model`, whereas [coerce] requires corruption when idealizing;
+/// hence the two may be callable on the same indexes.
+///
+/// We must have [create i a == coerce i a (sample (len a))]
+/// we currently check by hand that this follows from F* semantics.
+
+
+/// Derived key length restriction when using HKDF
+type keylen = l:UInt32.t {UInt32.v l <= 256}
+
+
+(* Definedness *)
+
+// Framing of package invariants can be done w.r.t either a region that is
+// disjoint from tls_define_region, or a define table that must be at a
+// different address than the package's define_table
+noeq type pkg_inv_r =
+  | Pinv_region: r:HH.rid{r `HH.disjoint` tls_define_region} -> pkg_inv_r
+  | Pinv_define: #it:eqtype -> #vt:(it -> Type) -> t:mem_table vt -> pkg_inv_r
+
+// When calling create or coerce, the footprint of a package grows only with
+// fresh subregions
+type modifies_footprint (fp:mem->GTot rset) h0 h1 =
+  forall (r:HH.rid). (Set.mem r (fp h0) /\ ~(Set.mem r (fp h1))) ==> stronger_fresh_region r h0 h1  //AR: 12/05: Could use the pattern {:pattern (Set.mem r (fp h0)); (Set.mem r (fp h1))}
+
+noeq type pkg (ip: ipkg) = | Pkg:
+  key: (i:ip.t {ip.registered i} -> Type0)  (* indexed state of the functionality *) ->
+  $info: (ip.t -> Type0)                    (* creation-time arguments, typically refined using i:ip.t *) ->
+  len: (#i:ip.t -> info i -> keylen)        (* computes the key-material length from those arguments *) ->
+  ideal: Type0                              (* type-level access to the ideal flag of the package *) ->
+  //17-11-13 do we need to know that ideal ==> model?
+  //17-11-13 is type-level access enough?
+
+  // when modelling, we maintain a global table of all allocated
+  // instances of the package. Only the package modifies the table.
+  //
+  // The package footprint is a function of the table contents;
+  // that collects all global and instance-local regions, but not [define_table]
+  define_table: mem_table #(i:ip.t {ip.registered i}) key ->
+  footprint: (mem -> GTot rset) ->
+  footprint_framing: (h0:mem -> h1:mem -> Lemma
+    (requires mem_stable define_table h0 h1)
+    (ensures footprint h0 == footprint h1)) ->
+
+  // we maintain a package invariant,
+  // which only depends on the table and footpring.
+  package_invariant: (mem -> Type0) ->
+  package_invariant_framing: (h0:mem -> r:pkg_inv_r -> h1:mem -> Lemma
+    (requires package_invariant h0 /\ mem_contains define_table h0 /\
+      (match r with
+      | Pinv_region r -> modifies_one r h0 h1 /\ ~(Set.mem r (footprint h0))
+      | Pinv_define #it #vt t ->
+        mem_contains t h0 /\ modifies_mem_table t h0 h1 /\ mem_disjoint t define_table))
+    (ensures package_invariant h1)) ->
+
+  // create and coerce, with a shared post-condition and framing lemma
+  // so that [derive] can pass the post-condition to its caller; the
+  // concrete part of the postcondition is what we need in [derive].
+  post: (#i:ip.t{ip.registered i} -> info i -> key i -> mem -> GTot Type0) ->
+  post_framing: (#i:ip.t{ip.registered i} -> a:info i -> k:key i ->  h0:mem -> r:HH.rid -> h1:mem -> Lemma
+     (requires (post a k h0 /\ modifies_one r h0 h1 /\ ~(r `Set.mem` footprint h0)))
+     (ensures (post a k h1))) ->
+
+  create: (i:ip.t{ip.registered i} -> a:info i -> ST (key i)
+    (requires fun h0 ->
+      model /\
+      package_invariant h0 /\
+      mem_fresh define_table i h0)
+    (ensures fun h0 k h1 ->
+      post a k h1 /\ package_invariant h1 /\
+      modifies_mem_table define_table h0 h1 /\
+      modifies_footprint footprint h0 h1 /\
+      mem_update define_table i k h0 h1)) ->
+
+  coerceT: (i:ip.t{ip.registered i /\ (ideal ==> ~(ip.honest i))} -> a:info i -> lbytes (len a) -> GTot (key i)) ->
+  coerce: (i:ip.t{ip.registered i /\ (ideal ==> ~(ip.honest i))} -> a:info i -> rk:lbytes (len a) -> ST (key i)
+    (requires fun h0 ->
+      package_invariant h0 /\
+      mem_fresh define_table i h0)
+    (ensures fun h0 k h1 ->
+      k == coerceT i a rk /\
+      post a k h1 /\ package_invariant h1 /\
+      modifies_mem_table define_table h0 h1 /\
+      modifies_footprint footprint h0 h1 /\
+      mem_update define_table i k h0 h1)) ->
+  pkg ip
+
+type fresh_regions (s:rset) (h0:mem) (h1:mem) =
+  forall (r:HH.rid).{:pattern (Set.mem r s)} Set.mem r s ==>
+    (stronger_fresh_region r h0 h1 \/ is_tls_rgn r)
+
+/// packages of instances with local private state, before ensuring
+/// their unique definition at every index and the disjointness of
+/// their footprints.
+noeq type local_pkg (ip: ipkg) =
+| LocalPkg:
+  $key: (i:ip.t{ip.registered i} -> Type0) ->
+  info: (ip.t -> Type0) ->
+  len: (#i:ip.t -> info i -> keylen) ->
+  ideal: Type0 ->
+  (* regions that are shared accross instances of the functionality *)
+  shared_footprint: rset ->
+  (* regions that are specific to each instance and freshly allocated when the instance is created *)
+  local_footprint: (#i:ip.t{ip.registered i} -> key i -> GTot (s:rset{s `Set.disjoint` shared_footprint})) ->
+  local_invariant: (#i:ip.t{ip.registered i} -> key i -> mem -> GTot Type0) (* instance invariant *) ->
+  local_invariant_framing: (i:ip.t{ip.registered i} -> k:key i -> h0:mem -> r:HH.rid -> h1:mem -> Lemma
+    (requires local_invariant k h0 /\ modifies_one r h0 h1
+      /\ ~(r `Set.mem` local_footprint k) /\ ~(r `Set.mem` shared_footprint))
+    (ensures local_invariant k h1)) ->
+  post: (#i:ip.t{ip.registered i} -> info i -> key i -> mem -> GTot Type0) ->
+  post_framing: (#i:ip.t{ip.registered i} -> a:info i -> k:key i -> h0:mem -> r:HH.rid -> h1:mem -> Lemma
+    (requires (post a k h0 /\ modifies_one r h0 h1 /\ ~(r `Set.mem` local_footprint k)))
+    (ensures (post a k h1))) ->
+  create: (i:ip.t{ip.registered i} -> a:info i -> ST (key i)
+    (requires fun h0 -> model)
+    (ensures fun h0 k h1 ->
+       modifies_none h0 h1 /\ local_invariant k h1 /\
+       post a k h1 /\ fresh_regions (local_footprint k) h0 h1)) ->
+  coerceT: (i:ip.t{ip.registered i /\ (ideal ==> ~(ip.honest i))} -> a:info i -> lbytes (len a) -> GTot (key i)) ->
+  coerce: (i:ip.t{ip.registered i /\ (ideal ==> ~(ip.honest i))} -> a:info i -> rk:lbytes (len a) -> ST (key i)
+    (requires fun h0 -> True)
+    (ensures fun h0 k h1 -> k == coerceT i a rk /\
+      modifies_none h0 h1 /\ local_invariant k h1 /\
+      post a k h1 /\ fresh_regions (local_footprint k) h0 h1)) ->
+  local_pkg ip
+
+(* Iterators over Monotonic.Map, require a change of implementation *)
+
+let mm_fold (#a:eqtype) (#b:a -> Type) (t:MM.map' a b)
+  (#rt:Type) (init:rt) (folder:rt -> i:a -> b i -> GTot rt) : GTot rt
+  = admit()
+
+let mm_fold_grow (#a:eqtype) (#b:a -> Type) (t:MM.map' a b) (t':MM.map' a b) (i:a) (v:b i)
+  (#rt:Type) (init:rt) (folder:rt -> i:a -> b i -> GTot rt) : Lemma
+  (requires t' == MM.upd t i v)
+  (ensures mm_fold t' init folder == folder (mm_fold t init folder) i v)
+  = admit()
+
+assume type mm_forall (#a:eqtype) (#b:a -> Type) (t:MM.map' a b)
+  (p: #i:a -> b i -> mem -> GTot Type0) (h:mem)
+
+let lemma_mm_forall_frame (#a:eqtype) (#b:a -> Type) (t:MM.map' a b)
+  (p: #i:a -> b i -> mem -> GTot Type0)
+  (footprint: #i:a -> v:b i -> GTot rset)
+  (p_frame: i:a -> v:b i -> h0:mem -> r:HH.rid -> h1:mem ->
+    Lemma (requires p v h0 /\ modifies_one r h0 h1 /\ ~(Set.mem r (footprint v)))
+          (ensures p v h1))
+  (r:HH.rid) (h0:mem) (h1:mem)
+  : Lemma (requires mm_forall t p h0 /\ modifies_one r h0 h1 /\
+            ~(Set.mem r (mm_fold t #rset Set.empty (fun s i k -> rset_union s (footprint k)))))
+          (ensures mm_forall t p h1)
+  = admit()
+
+let lemma_mm_forall_extend (#a:eqtype) (#b:a -> Type) (t:MM.map' a b) (t':MM.map' a b)
+  (p: #i:a -> b i -> mem -> GTot Type0) (i:a) (v:b i) (h0:mem) (h1:mem)
+  : Lemma (requires mm_forall t p h1 /\ t' == MM.upd t i v /\ p v h1)
+          (ensures mm_forall t' p h1)
+  = admit()
+
+let lemma_mm_forall_init (#a:eqtype) (#b:a -> Type) (t:MM.map' a b)
+  (p: #i:a -> b i -> mem -> GTot Type0) (h:mem)
+  : Lemma (requires t == MM.empty_map a b)
+          (ensures mm_forall t p h)
+  = admit()
+
+let lemma_mm_forall_elim (#a:eqtype) (#b:a -> Type) (t:MM.map' a b)
+  (p: #i:a -> b i -> mem -> GTot Type0) (i:a) (v:b i) (h:mem)
+  : Lemma (requires mm_forall t p h /\ t i == Some v)
+          (ensures p v h)
+  = admit()
+
+let lemma_union_com (s1:rset) (s2:rset) (s3:rset)
+  : Lemma (rset_union s1 (rset_union s2 s3) == rset_union (rset_union s1 s2) s3)
+  = admit()
+
+(* obsolete, replaced by refinement of memoize_ST
+unfold type mem_package (#ip:ipkg) (p:local_pkg ip) =
+  p':pkg ip{
+    Pkg?.key p' == LocalPkg?.key p /\
+    Pkg?.info p' == LocalPkg?.info p /\
+    Pkg?.len p' == LocalPkg?.len p /\
+    Pkg?.ideal p' == LocalPkg?.ideal p /\
+    (forall (#i:ip.t{ip.registered i}) (k:p.key i) (h:mem).
+      (mem_defined p'.define_table i /\ p'.package_invariant h) ==> p.local_invariant k h) /\
+    (forall (#i:ip.t{ip.registered i}) (a:p.info i) (k:p.key i) (h:mem).
+      (Pkg?.post p') #i (a <: Pkg?.info p' i) (k <: Pkg?.key p' i) h ==> (LocalPkg?.post p) #i a k h)
+  }
+*)
+
+// Memoization functor from local to global packages that memoize
+// instances produced by create/coerce and maintain their joint
+// invariant.
+//
+// We provide both a pure, unfolded functor and a stateful,
+// table-allocating functor; the latter is probably too opaque for
+// correlating its result with the source definitions.
+
+#set-options "--z3rlimit 100"
+//unfold
+let memoization (#ip:ipkg) (p:local_pkg ip) ($mtable: mem_table p.key): pkg ip =
+  let footprint_extend (s:rset) (i:ip.t{ip.registered i}) (k:p.key i) =
+    rset_union s (p.local_footprint k)
+    in
+  let footprint (h:mem): GTot rset =
+    let instances_footprint =
+      if model then
+        let map = MR.m_sel h (itable mtable) in
+        mm_fold map #rset Set.empty footprint_extend
+      else Set.empty in
+    rset_union p.shared_footprint instances_footprint
+    in
+  let footprint_grow (h0:mem) (i:ip.t{ip.registered i}) (k:p.key i) (h1:mem) : Lemma
+    (requires (mem_update mtable i k h0 h1 /\ fresh_regions (p.local_footprint k) h0 h1))
+    (ensures (modifies_footprint footprint h0 h1))
+    =
+    if model then
+     begin
+      let map = MR.m_sel h0 (itable mtable) in
+      let map' = MR.m_sel h1 (itable mtable) in
+      let fp0 = footprint h0 in
+      let fp1 = footprint h1 in
+      mm_fold_grow map map' i k #rset Set.empty footprint_extend;
+      assert(fp1 == rset_union p.shared_footprint (rset_union (mm_fold map #rset Set.empty footprint_extend) (p.local_footprint k)));
+      lemma_union_com p.shared_footprint (mm_fold map #rset Set.empty footprint_extend) (p.local_footprint k);
+      assert(fp1 == rset_union fp0 (p.local_footprint k));
+      assert(forall (r:HH.rid). (Set.mem r fp1 /\ ~(Set.mem r fp0)) ==> Set.mem r (p.local_footprint k));
+      assert(modifies_footprint footprint h0 h1)
+     end
+    else ()
+    in
+  let footprint_framing (h0:mem) (h1:mem) : Lemma
+    (requires mem_stable mtable h0 h1)
+    (ensures footprint h0 == footprint h1)
+    = ()
+  in
+  let package_invariant h =
+    (model ==>
+      (let log : i_mem_table p.key = itable mtable in
+      mm_forall (MR.m_sel h log) p.local_invariant h))
+    in
+  let ls_footprint (#i:ip.t{ip.registered i}) (k:p.key i) =
+    rset_union (p.local_footprint k) p.shared_footprint
+    in
+  let ls_footprint_frame (i:ip.t{ip.registered i}) (k:p.key i) (h0:mem) (r:HH.rid) (h1:mem)
+    : Lemma (requires p.local_invariant k h0 /\ modifies_one r h0 h1
+                      /\ ~(r `Set.mem` ls_footprint k))
+            (ensures p.local_invariant k h1)
+    =
+    assert(~(r `Set.mem` ls_footprint k) <==> ~(r `Set.mem` p.local_footprint k) /\ ~(r `Set.mem` p.shared_footprint));
+    p.local_invariant_framing i k h0 r h1
+    in
+  let package_invariant_framing (h0:mem) (r:pkg_inv_r) (h1:mem) : Lemma
+    (requires package_invariant h0 /\ mem_contains mtable h0 /\
+      (match r with
+      | Pinv_region r -> modifies_one r h0 h1 /\ ~(Set.mem r (footprint h0))
+      | Pinv_define #it #vt t -> mem_contains t h0 /\ modifies_mem_table t h0 h1 /\ mem_disjoint t mtable))
+    (ensures package_invariant h1)
+  =
+    if model then
+      let map = MR.m_sel h0 (itable mtable) in
+      assert(mm_forall map p.local_invariant h0);
+      (match r with
+      | Pinv_region r ->
+        assert(modifies_one r h0 h1 /\ r `HH.disjoint` tls_define_region);
+        lemma_mm_forall_frame map p.local_invariant ls_footprint ls_footprint_frame r h0 h1;
+        lemma_mem_frame mtable h0 r h1
+      | Pinv_define t ->
+        assert(modifies_mem_table t h0 h1 /\ mem_disjoint t mtable);
+        lemma_mm_forall_frame map p.local_invariant ls_footprint ls_footprint_frame tls_define_region h0 h1;
+        lemma_mem_disjoint_stable t mtable h0 h1)
+    else () in
+  let create (i:ip.t{ip.registered i}) (a:p.info i) : ST (p.key i)
+    (requires fun h0 -> model /\ package_invariant h0 /\ mem_fresh mtable i h0)
+    (ensures fun h0 k h1 -> modifies_mem_table mtable h0 h1
+      /\ modifies_footprint footprint h0 h1 /\ p.post a k h1
+      /\ package_invariant h1 /\ mem_update mtable i k h0 h1)
+    =
+    let h0 = get () in
+    let tbl : i_mem_table p.key = itable mtable in
+    MR.m_recall tbl;
+    let k : p.key i = p.create i a in
+    let h1 = get() in
+    assert(MR.m_sel h0 tbl == MR.m_sel h1 tbl);
+    package_invariant_framing h0 (Pinv_region tls_tables_region) h1;
+    MM.extend tbl i k;
+    let h2 = get () in
+    lemma_define_tls_honest_regions (p.local_footprint k);
+    p.post_framing #i a k h1 tls_define_region h2;
+    lemma_mm_forall_frame (MR.m_sel h1 tbl) p.local_invariant ls_footprint ls_footprint_frame tls_define_region h1 h2;
+    p.local_invariant_framing i k h1 tls_define_region h2;
+    lemma_mm_forall_extend (MR.m_sel h1 tbl) (MR.m_sel h2 tbl) p.local_invariant i k h1 h2;
+    assume(HS.modifies_ref tls_define_region (Set.singleton (mem_addr (itable mtable))) h0 h2); // How to prove?
+    footprint_grow h0 i k h2;
+    k in
+  let coerce (i:ip.t{ip.registered i /\ (p.ideal ==> ~(ip.honest i))}) (a:p.info i) (k0:lbytes (p.len a))
+    : ST (p.key i)
+    (requires fun h0 -> package_invariant h0 /\ mem_fresh mtable i h0)
+    (ensures fun h0 k h1 -> k == p.coerceT i a k0
+      /\ modifies_mem_table mtable h0 h1
+      /\ modifies_footprint footprint h0 h1 /\ p.post a k h1
+      /\ package_invariant h1 /\ mem_update mtable i k h0 h1)
+    =
+    if model then (
+      let h0 = get () in
+      let tbl : i_mem_table p.key = itable mtable in
+      MR.m_recall tbl;
+      let k : p.key i = p.coerce i a k0 in
+      let h1 = get() in
+      assert(MR.m_sel h0 tbl == MR.m_sel h1 tbl);
+      package_invariant_framing h0 (Pinv_region tls_tables_region) h1;
+      MM.extend tbl i k;
+      let h2 = get () in
+      lemma_define_tls_honest_regions (p.local_footprint k);
+      p.post_framing #i a k h1 tls_define_region h2;
+      lemma_mm_forall_frame (MR.m_sel h1 tbl) p.local_invariant ls_footprint ls_footprint_frame tls_define_region h1 h2;
+      p.local_invariant_framing i k h1 tls_define_region h2;
+      lemma_mm_forall_extend (MR.m_sel h1 tbl) (MR.m_sel h2 tbl) p.local_invariant i k h1 h2;
+      assume(HS.modifies_ref tls_define_region (Set.singleton (mem_addr (itable mtable))) h0 h2); // How to prove?
+      footprint_grow h0 i k h2;
+      k
+    ) else p.coerce i a k0
+    in
+  let post_framing (#i:ip.t{ip.registered i}) (a:p.info i) (k:p.key i)
+    (h0:mem) (r:HH.rid) (h1:mem) : Lemma
+    (requires p.post a k h0 /\ modifies_one r h0 h1 /\ ~(Set.mem r (footprint h0)))
+    (ensures p.post a k h1)
+    =
+    // FIXME(adl): we have a problem when model is false - we have nowhere to store
+    // the joint footprint of the concrete state! for now we will assume
+    // not model ==> local_footprint k = Set.empty for all k
+    // We may have to maintain an erased (i_mem_table p.key) when model is off to
+    // store the concrete footprints
+    assume(~(Set.mem r (footprint h0)) ==> ~(Set.mem r (p.local_footprint k)));
+    p.post_framing #i a k h0 r h1
+    in
+  (Pkg
+    p.key
+    p.info
+    p.len
+    p.ideal
+    mtable footprint footprint_framing
+    package_invariant package_invariant_framing
+    p.post post_framing
+    create p.coerceT coerce)
+
+let memoization_ST (#ip:ipkg) (p:local_pkg ip)
+  : ST (pkg ip)
+  (requires fun h0 -> True)
+  (ensures fun h0 q h1 ->
+    LocalPkg?.key p == Pkg?.key q /\ // seems to help
+    (let t: mem_table p.key = q.define_table in
+    modifies_mem_table t h0 h1 /\
+    q == memoization #ip p t /\
+    q.package_invariant h1))
+=
+  let h0 = get() in
+  let mtable: mem_table p.key = mem_alloc #(i:ip.t{ip.registered i}) p.key in
+  let h1 = get() in
+  let q = memoization #ip p mtable in
+  //assert(q == memoization #ip p mtable); // fails when unfolding memoization AR: 12/05: this is no longer needed per the new inlining behavior
+  // assert_norm(q == memoization #ip p mtable);// also fails, with squashing error
+  (if model then lemma_mm_forall_init (MR.m_sel h1 (itable mtable)) p.local_invariant h1);
+  q
+
